Assume lambdas has been removed through expansion

books/projects/smtlink/verified/process.lisp
@@ -18,201 +18,90 @@
 (include-book "evaluator")
 (include-book "../config")
 
-(defsection Smtlink-process-user-hint
-  :parents (verified)
-  :short "Functionalities for processing user hints given to Smtlink. User
-  hints will be merged with (smt-hint)."
+;; (defsection Smtlink-process-user-hint
+;;   :parents (verified)
+;;   :short "Functionalities for processing user hints given to Smtlink. User
+;;   hints will be merged with (smt-hint)."
 
   ;; --------------------------------------------------------
 
 ;; Example:
 ;; :hints (("Goal"
-;;          :smtlink
-;;          (:functions
-;;           ((f0 :formals ((a0 rationalp))
-;;                :returns
-;;                ((r0 rationalp
-;;                     :name rationalp-of-f0))
-;;                :expansion-depth 1
-;;                :guard ((> a0 0)
-;;                        :name a0->-0 <or>
-;;                        :hints (:use ((:instance guard-lemma))))
-;;                :more-returns
-;;                (((> r0 0)
-;;                  :name r0->-0 <or> :hints (:use ((:instance more-lemma)))))))
-;;           :types
-;;           ((integer-list
-;;             :recognizer integer-listp
-;;             :fixer integer-list-fix
-;;             :fixer-when-recognizer-thm integer-list-fix-when-integer-listp
-;;             :kind (:list
-;;                    :cons
-;;                    (:constructor
-;;                     (integer-list-cons :return-type integer-list-p
-;;                                        :type-thm (:name ... :hints ...))
-;;                     :destructors
-;;                     ((integer-list-car :return-type integerp
-;;                                        :type-thm (:name ...)
-;;                                        :destructor-thm (:name ...))
-;;                      (integer-list-cdr ...)))
-;;                    :nil-kind
-;;                    (:constructor
-;;                     (integer-list-nil :return-type ...
-;;                                       :type-thm (:name ... :hints ...))))
-;;             (:abstract)
-;;             (:prod
-;;              :constructor ()
-;;              :destructors (() () ...))
-;;             (:sum
-;;              :kind-fn integer-list-kind
-;;              :kind1
-;;              (:constructor (...)
-;;               :destructors (() () ...))
-;;              :kind2
-;;               (:constructor (...)
-;;                :destructors (() () ...)))
-;;             (:option
-;;              :some
-;;              (:constructor ()
-;;               :destructor ())
-;;              :none
-;;              (:constructor ()))
-;;            (...)
-;;            ...)
-;;           :hypotheses (((> a b) :hints (:use ((:instance lemma)))))
-;;           :rm-file t
-;;           :smt-dir ""
-;;           :smt-fname ""
-;;           :int-to-rat nil
-;;           :use-uninterpreted t
-;;           :under-induct nil
-;;           :global-hint nil
-;;           :wrld-fn-len 0
-;;           :custom-p nil
-;;           )))
+;;            :clause-processor
+;;            (SMT::smtlink clause
+;;                          '(:functions ((f0 :formals (x y)
+;;                                            :return ((r :thm returns-thm)
+;;                                                     (r :thm another-returns-thm))
+;;                                            :uninterpreted-hints ((:use lemma))
+;;                                            :replace replace-thm
+;;                                            :depth 1))
+;;                            :hypotheses ((:instance thm1 ((x (1+ (foo a))) (y n)))
+;;                                         (:instance thm2 ...))
+;;                            :types ((rational-listp
+;;                                     :functions
+;;                                     ((rational-list-fix
+;;                                       :formals (lst)
+;;                                       :returns (x :thm returns-thm)
+;;                                       :replace replace-thm)
+;;                                      (rational-list-car
+;;                                       :formals (lst)
+;;                                       :returns (x :thm returns-thm)
+;;                                       :replace replace-thm)
+;;                                      (rational-list-cdr
+;;                                       :formals (lst)
+;;                                       :returns (x :thm returns-thm)
+;;                                       :replace replace-thm)
+;;                                      (rational-list-cons
+;;                                       :formals (x lst)
+;;                                       :returns (xlst :thm returns-thm)
+;;                                       :replace replace-thm))
+;;                                     :subtypes (integer-listp)))
+;;                            :int-to-ratp (x b)
+;;                            :under-inductionp t
+;;                            :smt-fname ""
+;;                            :rm-file t
+;;                            :global-hint current-hint
+;;                            :customp nil))))
+;;   )
 
-  ;; A few note for :name of hint-pair:
-  ;; A :name represents the name of the theorem. This theorem when
-  ;; instantiated can be used as a conjunction of the hypotheses and this can
-  ;; be proved using meta-extract, so no additional subgoals will be generated.
-  ;; When a :hints used, it gives an ACL2 hint that can help with the proof of
-  ;; the generated subgoal.
-  ;;
-  ;; In principal, Smtlink returns the minimal number of subgoals, therefore
-  ;; :name should be in most cases the only one that's useful. I'm keeping
-  ;; :hints in case we do need it in some cases.
-  ;;
-  ;; When both :name and :hints exist, :name is preferred.
-  ;;
-
-  ;; TODO: implement use-uninterpreted and under-induct options
-  ;; TODO: I will write macros for this file if I've got time.
-  )
-
-(defsection hints-syntax
+(defsection hypothesis-list-syntax
   :parents (Smtlink-process-user-hint)
 
-  (define hints-syntax-p ((term t))
+  (define subst-syntax-p ((subst t))
     :returns (syntax-good? booleanp)
-    :short "Recognizer for hints-syntax."
-    (true-listp term)
-    ///
-    (more-returns
-     (syntax-good?
-      (implies syntax-good? (true-listp term))
-      :name true-listp-of-hints-syntax-p)))
+    (b* (((unless (consp subst)) (null subst))
+         ((cons subst-hd subst-tl) subst)
+         (res-hd
+          (case-match subst-hd
+            ((var term) (and (symbolp var) (pseudo-termp term)))
+            (& nil))))
+      (and res-hd (subst-syntax-p subst-tl))))
 
-  (easy-fix hints-syntax nil)
-  )
-
-(defsection hypothesis-lst-syntax
-  :parents (Smtlink-process-user-hint)
+  (easy-fix subst-syntax 'nil)
 
   (define hypothesis-syntax-p ((term t))
     :returns (syntax-good? booleanp)
     :short "Recognizer for hypothesis-syntax."
-    (or (and (atom term)
-             (equal term nil))
-        ;; Without hints
-        (and (true-listp term)
-             (car term) (not (cdr term))
-             (pseudo-termp (car term)))
-        ;; With name
-        (and (true-listp term)
-             (car term) (cadr term) (not (cdddr term))
-             (pseudo-termp (car term))
-             (equal (cadr term) ':name)
-             (symbolp (caddr term)))
-        ;; With hints
-        (and (true-listp term)
-             (car term) (cadr term) (not (cdddr term))
-             (pseudo-termp (car term))
-             (equal (cadr term) ':hints)
-             (hints-syntax-p (caddr term))))
-    ///
-    (defthm true-listp-of-caddr
-      (implies
-       (and (consp term)
-            (consp (cdr term))
-            (true-listp (cddr term))
-            (equal (+ 2 (len (cddr term))) 3)
-            (pseudo-termp (car term))
-            (equal (cadr term) :hints)
-            (hints-syntax-p (caddr term)))
-       (true-listp (caddr term)))
-      :hints (("Goal" :in-theory (enable hints-syntax-p))))
-    )
+    (or (and (consp term)
+             (consp (cdr term))
+             (null (cddr term))
+             (equal (car term) :instance)
+             (symbolp (cadr term)))
+        (and (consp term)
+             (consp (cdr term))
+             (consp (cddr term))
+             (null (cdddr term))
+             (equal (car term) :instance)
+             (symbolp (cadr term))
+             (subst-syntax-p (caddr term)))))
 
-  (easy-fix hypothesis-syntax nil)
+  (easy-fix hypothesis-syntax '(:instance nil))
 
-  (deflist hypothesis-lst-syntax
-    :pred hypothesis-lst-syntax-p
+  (deflist hypothesis-list-syntax
+    :pred hypothesis-list-syntax-p
     :elt-type hypothesis-syntax-p
     :true-listp t)
 )
-
-(defsection argument-lst-syntax
-  :parents (Smtlink-process-user-hint)
-
-  (define smt-typep ((term t))
-    :enabled t
-    :returns (valid-type? booleanp)
-    :short "Should be a smtlink fixtype. This is just a syntax check, so it
-    only need to be a symbol."
-    (symbolp term))
-
-  (define argument-syntax-p ((term t))
-    :returns (syntax-good? booleanp)
-    :short "recognizer for argument-syntax."
-    (or (and (atom term)
-             (equal term nil))
-        ;; just the name
-        (and (true-listp term)
-             (car term) (not (cdr term))
-             (symbolp (car term)))
-        ;; the name and the type/guard
-        (and (true-listp term)
-             (car term) (cadr term) (not (cddr term))
-             (symbolp (car term))
-             (smt-typep (cadr term)))
-        ;; the name, the type and the theorem
-        ;; For formals, no such theorem exists;
-        ;; For returns, such theorem exists
-        (and (true-listp term)
-             (car term) (cadr term) (not (cddddr term))
-             (symbolp (car term))
-             (smt-typep (cadr term))
-             (equal ':name (caddr term))
-             (symbolp (cadddr term)))
-        ))
-
-  (easy-fix argument-syntax nil)
-
-  (deflist argument-lst-syntax
-    :elt-type argument-syntax-p
-    :pred argument-lst-syntax-p
-    :true-listp t)
-  )
 
 (defthm symbol-list-fix-preserve-member-equal
   (implies (and (consp x)
@@ -231,6 +120,25 @@
 (defsection function-option-syntax
   :parents (function-syntax)
 
+  (define return-syntax-p ((term t))
+    :returns (ok booleanp)
+    (case-match term
+      ((var ':thm thm) (and (symbolp var) (symbolp thm)))
+      (& nil)))
+
+  (easy-fix return-syntax '(nil :thm nil))
+
+  (define return-list-syntax-p ((term t))
+    :returns (ok booleanp)
+    :short "Return theorem list syntax."
+    (b* (((unless (or (consp term) (null term))) nil)
+         ((if (null term)) t)
+         ((cons return-hd return-tl) term))
+      (and (return-syntax-p return-hd)
+           (return-list-syntax-p return-tl))))
+
+  (easy-fix return-list-syntax nil)
+
   (define function-option-syntax-p-helper ((term t) (used symbol-listp))
     :returns (ok booleanp)
     :short "Helper function for function-option-syntax."
@@ -243,16 +151,15 @@
               "~p0 option is already defined in the hint.~%" first))
          (first-ok
           (case first
-            ;; TODO: I didn't check for distinct formals.
-            (:formals (argument-lst-syntax-p second))
-            (:returns (argument-lst-syntax-p second))
-            (:expansion-depth (natp second))
-            (:guard (hypothesis-syntax-p second))
-            (:more-returns (hypothesis-lst-syntax-p second))
+            (:formals (symbol-listp second))
+            (:return (return-list-syntax-p second))
+            (:uninterpreted-hints (true-listp second))
+            (:replace (symbolp second))
+            (:depth (natp second))
             (t (er hard? 'process=>function-option-syntax-p-helper
                    "Smtlink-hint function hint option doesn't include: ~p0.
-                       They are :formals, :returns, :expansion-depth, :guard, and
-                       :more-returns.~%" first)))))
+                       They are :formals, :return, :return-hints, :replace, and
+                       :depth.~%" first)))))
       (and first-ok
            (function-option-syntax-p-helper rest (cons first used))))
     ///
@@ -261,28 +168,27 @@
                   (and (not (member-equal (car term) used))
                        (consp (cdr term))
                        (implies (equal (car term) :formals)
-                                (argument-lst-syntax-p (cadr term)))
-                       (implies (equal (car term) :returns)
-                                (argument-lst-syntax-p (cadr term)))
-                       (implies (equal (car term) :expansion-depth)
-                                (natp (cadr term)))
-                       (implies (equal (car term) :guard)
-                                (hypothesis-syntax-p (cadr term)))
-                       (implies (equal (car term) :more-returns)
-                                (hypothesis-lst-syntax-p (cadr term)))))
+                                (symbol-listp (cadr term)))
+                       (implies (equal (car term) :return)
+                                (return-list-syntax-p (cadr term)))
+                       (implies (equal (car term) :uninterpreted-hints)
+                                (true-listp (cadr term)))
+                       (implies (equal (car term) :replace)
+                                (symbolp (cadr term)))
+                       (implies (equal (car term) :depth)
+                                (natp (cadr term)))))
          :name definition-of-function-option-syntax-p-helper)
      (ok (implies (and (symbol-listp used) ok (consp term))
                   (or (equal (car term) :formals)
-                      (equal (car term) :returns)
-                      (equal (car term) :guard)
-                      (equal (car term) :more-returns)
-                      (equal (car term) :expansion-depth)))
+                      (equal (car term) :return)
+                      (equal (car term) :uninterpreted-hints)
+                      (equal (car term) :replace)
+                      (equal (car term) :depth)))
          :name option-of-function-option-syntax-p-helper))
     (defthm monotonicity-of-function-option-syntax-p-helper
       (implies (and (subsetp used-1 used :test 'equal)
                     (function-option-syntax-p-helper term used))
-               (function-option-syntax-p-helper term used-1)))
-    )
+               (function-option-syntax-p-helper term used-1))))
 
   (defthm monotonicity-of-function-option-syntax-p-helper-corollary
     (implies (function-option-syntax-p-helper term used)
@@ -302,39 +208,35 @@
      (ok (implies (and ok (consp term))
                   (and (consp (cdr term))
                        (implies (equal (car term) :formals)
-                                (argument-lst-syntax-p (cadr term)))
-                       (implies (equal (car term) :returns)
-                                (argument-lst-syntax-p (cadr term)))
-                       (implies (equal (car term) :expansion-depth)
-                                (natp (cadr term)))
-                       (implies (equal (car term) :guard)
-                                (hypothesis-syntax-p (cadr term)))
-                       (implies (equal (car term) :more-returns)
-                                (hypothesis-lst-syntax-p (cadr term)))))
+                                (symbol-listp (cadr term)))
+                       (implies (equal (car term) :return)
+                                (return-list-syntax-p (cadr term)))
+                       (implies (equal (car term) :uninterpreted-hints)
+                                (true-listp (cadr term)))
+                       (implies (equal (car term) :replace)
+                                (symbolp (cadr term)))
+                       (implies (equal (car term) :depth)
+                                (natp (cadr term)))))
          :name definition-of-function-option-syntax-p
          :hints (("Goal"
                   :in-theory (disable definition-of-function-option-syntax-p-helper)
-                  :use ((:instance
-                         definition-of-function-option-syntax-p-helper
-                         (used nil))))))
+                  :use ((:instance definition-of-function-option-syntax-p-helper
+                                   (used nil))))))
      (ok (implies (and ok (consp term)
-                       (not (equal (car term) :expansion-depth))
                        (not (equal (car term) :formals))
-                       (not (equal (car term) :returns))
-                       (not(equal (car term) :guard)))
-                  (equal (car term) :more-returns))
+                       (not (equal (car term) :return))
+                       (not (equal (car term) :uninterpreted-hints))
+                       (not(equal (car term) :replace)))
+                  (equal (car term) :depth))
          :name option-of-function-option-syntax-p
          :hints (("Goal"
                   :in-theory (disable option-of-function-option-syntax-p-helper)
-                  :use ((:instance
-                         option-of-function-option-syntax-p-helper
-                         (used nil))))))
+                  :use ((:instance option-of-function-option-syntax-p-helper
+                                   (used nil))))))
      (ok (implies (and ok (consp term))
                   (function-option-syntax-p (cddr term)))
-         :hints (("Goal"
-                  :expand (function-option-syntax-p-helper term nil)))
-         :name monotonicity-of-function-option-syntax-p)
-     ))
+         :hints (("Goal" :expand (function-option-syntax-p-helper term nil)))
+         :name monotonicity-of-function-option-syntax-p)))
 
   (easy-fix function-option-syntax nil)
   )
@@ -353,655 +255,10 @@
 
   (easy-fix function-syntax nil)
 
-  (deflist function-lst-syntax
+  (deflist function-list-syntax
     :elt-type function-syntax-p
-    :pred function-lst-syntax-p
+    :pred function-list-syntax-p
     :true-listp t)
-  )
-
-(defsection type-function-syntax
-  :parents (kind-syntax)
-
-  (define type-thm-syntax-p-helper ((term t)
-                                    (used symbol-listp))
-    :returns (ok booleanp)
-    :short "Helper function for type-thm-syntax."
-    (b* ((used (symbol-list-fix used))
-         ((unless (consp term)) t)
-         ((unless (and (consp term) (consp (cdr term)))) nil)
-         ((list* first second rest) term)
-         ((if (member-equal first used))
-          (er hard? 'process=>type-thm-syntax-p-helper
-              "~p0 option is already defined in the hint.~%" first))
-         (first-ok
-          (case first
-            (:name (symbolp second))
-            (:hints (hints-syntax-p second))
-            (t (er hard? 'process=>type-thm-syntax-p-helper
-                   "Smtlink-hint type-thm-syntax option doesn't include:
-                    ~p0. They are :name, and :hints~%" first)))))
-      (and first-ok
-           (type-thm-syntax-p-helper rest (cons first used))))
-    ///
-    (more-returns
-     (ok (implies (and ok (consp term) (symbol-listp used))
-                  (and (consp (cdr term))
-                       (not (member-equal (car term) used))
-                       (implies (equal (car term) :name)
-                                (symbolp (cadr term)))
-                       (implies (equal (car term) :hints)
-                                (hints-syntax-p (cadr term)))))
-         :name definition-of-type-thm-syntax-p-helper
-         :hints (("Goal"
-                  :expand (type-thm-syntax-p-helper term used))))
-     (ok (implies (and ok (consp term) (symbol-listp used)
-                       (not (equal (car term) :name)))
-                  (equal (car term) :hints))
-         :name option-of-type-thm-syntax-p-helper
-         :hints (("Goal"
-                  :expand (type-thm-syntax-p-helper term used)))))
-     (defthm monotonicity-of-type-thm-syntax-p-helper
-       (implies (and (subsetp used-1 used :test 'equal)
-                     (type-thm-syntax-p-helper term used))
-                (type-thm-syntax-p-helper term used-1)))
-     )
-
-  (defthm monotonicity-of-type-thm-syntax-p-helper-corollary
-    (implies (type-thm-syntax-p-helper term used)
-             (type-thm-syntax-p-helper term nil))
-    :hints (("Goal"
-             :in-theory (disable monotonicity-of-type-thm-syntax-p-helper)
-             :use ((:instance monotonicity-of-type-thm-syntax-p-helper
-                              (used used)
-                              (used-1 nil))))))
-
-  (define type-thm-syntax-p ((term t))
-    :returns (ok booleanp)
-    :short "Recognizer for type-thm-syntax-p."
-    (type-thm-syntax-p-helper term nil)
-    ///
-    (more-returns
-     (ok (implies (and ok (consp term))
-                  (and (consp (cdr term))
-                       (implies (equal (car term) :name)
-                                (symbolp (cadr term)))
-                       (implies (equal (car term) :hints)
-                                (hints-syntax-p (cadr term)))))
-         :name definition-of-type-thm-syntax-p
-         :hints (("Goal"
-                  :in-theory (disable definition-of-type-thm-syntax-p-helper)
-                  :use ((:instance
-                         definition-of-type-thm-syntax-p-helper
-                         (used nil))))))
-     (ok (implies (and ok (consp term)
-                       (not (equal (car term) :name)))
-                  (equal (car term) :hints))
-         :name option-of-type-thm-syntax-p
-         :hints (("Goal"
-                  :in-theory (disable option-of-type-thm-syntax-p-helper)
-                  :use ((:instance
-                         option-of-type-thm-syntax-p-helper
-                         (used nil))))))
-     (ok (implies (and ok (consp term))
-                  (type-thm-syntax-p (cddr term)))
-         :hints (("Goal"
-                  :expand (type-thm-syntax-p-helper term nil)))
-         :name monotonicity-of-type-thm-syntax-p)
-     ))
-
-  (easy-fix type-thm-syntax nil)
-
-  (define type-function-option-syntax-p-helper ((term t)
-                                                (used symbol-listp))
-    :returns (ok booleanp)
-    :short "Helper function for type-function-option-syntax."
-    (b* ((used (symbol-list-fix used))
-         ((unless (consp term)) t)
-         ((unless (and (consp term) (consp (cdr term)))) nil)
-         ((list* first second rest) term)
-         ((if (member-equal first used))
-          (er hard? 'process=>type-function-option-syntax-p-helper
-              "~p0 option is already defined in the hint.~%" first))
-         (first-ok
-          (case first
-            (:return-type (symbolp second))
-            (:type-thm (type-thm-syntax-p second))
-            (:destructor-thm (type-thm-syntax-p second))
-            (t (er hard? 'process=>type-function-option-syntax-p-helper
-                   "Smtlink-hint type-function-option-syntax option doesn't
-                    include: ~p0. They are :return-type, :type-thm, and
-                    :destructor-thm.~%" first)))))
-      (and first-ok
-           (type-function-option-syntax-p-helper rest (cons first used))))
-    ///
-    (more-returns
-     (ok (implies (and ok (consp term) (symbol-listp used))
-                  (and (consp (cdr term))
-                       (not (member-equal (car term) used))
-                       (implies (equal (car term) :return-type)
-                                (symbolp (cadr term)))
-                       (implies (equal (car term) :type-thm)
-                                (type-thm-syntax-p (cadr term)))
-                       (implies (equal (car term) :destructor-thm)
-                                (type-thm-syntax-p (cadr term)))))
-         :name definition-of-type-function-option-syntax-p-helper
-         :hints (("Goal"
-                  :expand (type-function-option-syntax-p-helper term used))))
-     (ok (implies (and ok (consp term) (symbol-listp used)
-                       (not (equal (car term) :return-type))
-                       (not (equal (car term) :type-thm)))
-                  (equal (car term) :destructor-thm))
-         :name option-of-type-function-option-syntax-p-helper
-         :hints (("Goal"
-                  :expand (type-function-option-syntax-p-helper term used)))))
-    (defthm monotonicity-of-type-function-option-syntax-p-helper
-      (implies (and (subsetp used-1 used :test 'equal)
-                    (type-function-option-syntax-p-helper term used))
-               (type-function-option-syntax-p-helper term used-1))))
-
-  (defthm monotonicity-of-type-function-option-syntax-p-helper-corollary
-    (implies (type-function-option-syntax-p-helper term used)
-             (type-function-option-syntax-p-helper term nil))
-    :hints (("Goal"
-             :in-theory (disable monotonicity-of-type-function-option-syntax-p-helper)
-             :use ((:instance monotonicity-of-type-function-option-syntax-p-helper
-                              (used used)
-                              (used-1 nil))))))
-
-  (define type-function-option-syntax-p ((term t))
-    :returns (ok booleanp)
-    :short "Recognizer for type-function-option-syntax-p."
-    (type-function-option-syntax-p-helper term nil)
-    ///
-    (more-returns
-     (ok (implies (and ok (consp term))
-                  (and (consp (cdr term))
-                       (implies (equal (car term) :return-type)
-                                (symbolp (cadr term)))
-                       (implies (equal (car term) :type-thm)
-                                (type-thm-syntax-p (cadr term)))
-                       (implies (equal (car term) :destructor-thm)
-                                (type-thm-syntax-p (cadr term)))))
-         :name definition-of-type-function-option-syntax-p
-         :hints (("Goal"
-                  :in-theory (disable definition-of-type-function-option-syntax-p-helper)
-                  :use ((:instance
-                         definition-of-type-function-option-syntax-p-helper
-                         (used nil))))))
-     (ok (implies (and ok (consp term)
-                       (not (equal (car term) :return-type))
-                       (not (equal (car term) :type-thm)))
-                  (equal (car term) :destructor-thm))
-         :name option-of-type-function-option-syntax-p
-         :hints (("Goal"
-                  :in-theory (disable option-of-type-function-option-syntax-p-helper)
-                  :use ((:instance
-                         option-of-type-function-option-syntax-p-helper
-                         (used nil))))))
-     (ok (implies (and ok (consp term))
-                  (type-function-option-syntax-p (cddr term)))
-         :hints (("Goal"
-                  :expand (type-function-option-syntax-p-helper term nil)))
-         :name monotonicity-of-type-function-option-syntax-p)))
-
-  (easy-fix type-function-option-syntax nil)
-
-  (define type-function-syntax-p ((term t))
-    :returns (ok booleanp)
-    :short "Recognizer for type-function-syntax-p."
-    (b* (((unless (consp term)) nil)
-         ((cons name options) term))
-      (and (symbolp name)
-           (type-function-option-syntax-p options))))
-
-  (easy-fix type-function-syntax '(:abstract))
-
-  (deflist type-function-list-syntax
-    :elt-type type-function-syntax-p
-    :true-listp t)
-  )
-
-(defsection kind-syntax
-  :parents (type-syntax)
-
-  ;; abstract-kind
-  (define abstract-kind-syntax-p ((term t))
-    :returns (ok booleanp)
-    :short "Recoginizer for abstract-kind-syntax."
-    (null term))
-
-  (easy-fix abstract-kind-syntax nil)
-
-  ;; array-kind
-  (define array-kind-syntax-p-helper ((term t) (used symbol-listp))
-    :returns (ok booleanp)
-    :short "Helper function for array-kind-syntax."
-    (b* ((used (symbol-list-fix used))
-         ((unless (consp term)) t)
-         ((unless (and (consp term) (consp (cdr term)))) nil)
-         ((list* first second rest) term)
-         ((if (member-equal first used))
-          (er hard? 'process=>array-kind-syntax-p-helper
-              "~p0 option is already defined in the hint.~%" first))
-         (first-ok
-          (case first
-            (:store (symbolp second))
-            (:select (symbolp second))
-            (:k (symbolp second))
-            (:key-type (symbolp second))
-            (:val-type (symbolp second))
-            (:array-thm (type-thm-syntax-p second))
-            (t (er hard? 'process=>array-kind-syntax-p-helper
-                   "Smtlink-hint array-kind option doesn't include: ~p0.
-                       They are :store, :select, :k, :key-type, :val-type, and
-                       :array-thm.~%" first)))))
-      (and first-ok
-           (array-kind-syntax-p-helper rest (cons first used)))))
-
-  (define array-kind-syntax-p ((term t))
-    :returns (ok booleanp)
-    :short "Recoginizer for array-kind-syntax."
-    (array-kind-syntax-p-helper term nil))
-
-  (easy-fix array-kind-syntax nil)
-
-  ;; prod-option
-  (define prod-option-syntax-p-helper ((term t) (used symbol-listp))
-    :returns (ok booleanp)
-    :short "Helper function for prod-option-syntax."
-    (b* ((used (symbol-list-fix used))
-         ((unless (consp term)) t)
-         ((unless (and (consp term) (consp (cdr term)))) nil)
-         ((list* first second rest) term)
-         ((if (member-equal first used))
-          (er hard? 'process=>prod-option-syntax-p-helper
-              "~p0 option is already defined in the hint.~%" first))
-         (first-ok
-          (case first
-            (:constructor (type-function-syntax-p second))
-            (:destructors (type-function-list-syntax-p second))
-            (t (er hard? 'process=>prod-option-syntax-p-helper
-                   "Smtlink-hint prod-option doesn't include: ~p0.
-                       They are :constructor, and :field-accessors.~%"
-                   first)))))
-      (and first-ok
-           (prod-option-syntax-p-helper rest (cons first used))))
-    ///
-    (more-returns
-     (ok (implies (and ok (consp term) (symbol-listp used))
-                  (and (consp (cdr term))
-                       (not (member-equal (car term) used))
-                       (implies (equal (car term) :constructor)
-                                (type-function-syntax-p (cadr term)))
-                       (implies (equal (car term) :destructors)
-                                (type-function-list-syntax-p (cadr term)))))
-         :name definition-of-prod-option-syntax-p-helper
-         :hints (("Goal"
-                  :expand (prod-option-syntax-p-helper term used))))
-     (ok (implies (and ok (consp term) (symbol-listp used)
-                       (not (equal (car term) :constructor)))
-                  (equal (car term) :destructors))
-         :name option-of-prod-option-syntax-p-helper
-         :hints (("Goal"
-                  :expand (prod-option-syntax-p-helper term used)))))
-    (defthm monotonicity-of-prod-option-syntax-p-helper
-      (implies (and (subsetp used-1 used :test 'equal)
-                    (prod-option-syntax-p-helper term used))
-               (prod-option-syntax-p-helper term used-1))))
-
-  (defthm monotonicity-of-prod-option-syntax-p-helper-corollary
-    (implies (prod-option-syntax-p-helper term used)
-             (prod-option-syntax-p-helper term nil))
-    :hints (("Goal"
-             :in-theory (disable monotonicity-of-prod-option-syntax-p-helper)
-             :use ((:instance monotonicity-of-prod-option-syntax-p-helper
-                              (used used)
-                              (used-1 nil))))))
-
-  (define prod-kind-syntax-p ((term t))
-    :returns (ok booleanp)
-    :short "Recognizer for prod-kind-syntax."
-    (prod-option-syntax-p-helper term nil)
-    ///
-    (more-returns
-     (ok (implies (and ok (consp term))
-                  (and (consp (cdr term))
-                       (implies (equal (car term) :constructor)
-                                (type-function-syntax-p (cadr term)))
-                       (implies (equal (car term) :destructors)
-                                (type-function-list-syntax-p (cadr term)))))
-         :name definition-of-prod-kind-syntax-p
-         :hints (("Goal"
-                  :in-theory (disable definition-of-prod-option-syntax-p-helper)
-                  :use ((:instance
-                         definition-of-prod-option-syntax-p-helper
-                         (used nil))))))
-     (ok (implies (and ok (consp term)
-                       (not (equal (car term) :constructor)))
-                  (equal (car term) :destructors))
-         :name option-of-prod-kind-syntax-p
-         :hints (("Goal"
-                  :in-theory (disable option-of-prod-option-syntax-p-helper)
-                  :use ((:instance
-                         option-of-prod-option-syntax-p-helper
-                         (used nil))))))
-     (ok (implies (and ok (consp term))
-                  (prod-kind-syntax-p (cddr term)))
-         :hints (("Goal"
-                  :expand (prod-option-syntax-p-helper term nil)))
-         :name monotonicity-of-prod-kind-syntax-p)))
-
-  (easy-fix prod-kind-syntax nil)
-
-  ;; list-kind
-  (define list-kind-syntax-p-helper ((term t) (used symbol-listp))
-    :returns (ok booleanp)
-    :short "Helper function for list-kind-syntax."
-    (b* ((used (symbol-list-fix used))
-         ((unless (consp term)) t)
-         ((unless (and (consp term) (consp (cdr term)))) nil)
-         ((list* first second rest) term)
-         ((if (member-equal first used))
-          (er hard? 'process=>list-kind-syntax-p-helper
-              "~p0 option is already defined in the hint.~%" first))
-         (first-ok
-          (case first
-            (:cons (prod-kind-syntax-p second))
-            (:nil-kind (prod-kind-syntax-p second))
-            (t (er hard? 'process=>list-kind-syntax-p-helper
-                   "Smtlink-hint list-kind option doesn't include: ~p0.
-                       They are :cons, and :nil-kind.~%"
-                   first)))))
-      (and first-ok
-           (list-kind-syntax-p-helper rest (cons first used))))
-    ///
-    (more-returns
-     (ok (implies (and ok (consp term) (symbol-listp used))
-                  (and (consp (cdr term))
-                       (not (member-equal (car term) used))
-                       (implies (equal (car term) :cons)
-                                (prod-kind-syntax-p (cadr term)))
-                       (implies (equal (car term) :nil-kind)
-                                (prod-kind-syntax-p (cadr term)))))
-         :name definition-of-list-kind-syntax-p-helper
-         :hints (("Goal"
-                  :expand (list-kind-syntax-p-helper term used))))
-     (ok (implies (and ok (consp term) (symbol-listp used)
-                       (not (equal (car term) :cons)))
-                  (equal (car term) :nil-kind))
-         :name option-of-list-kind-syntax-p-helper
-         :hints (("Goal"
-                  :expand (list-kind-syntax-p-helper term used)))))
-    (defthm monotonicity-of-list-kind-syntax-p-helper
-      (implies (and (subsetp used-1 used :test 'equal)
-                    (list-kind-syntax-p-helper term used))
-               (list-kind-syntax-p-helper term used-1))))
-
-  (defthm monotonicity-of-list-kind-syntax-p-helper-corollary
-    (implies (list-kind-syntax-p-helper term used)
-             (list-kind-syntax-p-helper term nil))
-    :hints (("Goal"
-             :in-theory (disable monotonicity-of-list-kind-syntax-p-helper)
-             :use ((:instance monotonicity-of-list-kind-syntax-p-helper
-                              (used used)
-                              (used-1 nil))))))
-
-  (define list-kind-syntax-p ((term t))
-    :returns (ok booleanp)
-    :short "Recognizer for list-kind-syntax."
-    (list-kind-syntax-p-helper term nil)
-    ///
-    (more-returns
-     (ok (implies (and ok (consp term))
-                  (and (consp (cdr term))
-                       (implies (equal (car term) :cons)
-                                (prod-kind-syntax-p (cadr term)))
-                       (implies (equal (car term) :nil-kind)
-                                (prod-kind-syntax-p (cadr term)))))
-         :name definition-of-list-kind-syntax-p
-         :hints (("Goal"
-                  :in-theory (disable definition-of-list-kind-syntax-p-helper)
-                  :use ((:instance
-                         definition-of-list-kind-syntax-p-helper
-                         (used nil))))))
-     (ok (implies (and ok (consp term)
-                       (not (equal (car term) :cons)))
-                  (equal (car term) :nil-kind))
-         :name option-of-list-kind-syntax-p
-         :hints (("Goal"
-                  :in-theory (disable option-of-list-kind-syntax-p-helper)
-                  :use ((:instance
-                         option-of-list-kind-syntax-p-helper
-                         (used nil))))))
-     (ok (implies (and ok (consp term))
-                  (list-kind-syntax-p (cddr term)))
-         :hints (("Goal"
-                  :expand (list-kind-syntax-p-helper term nil)))
-         :name monotonicity-of-list-kind-syntax-p)))
-
-  (easy-fix list-kind-syntax nil)
-
-  ;; option-kind
-  (define option-kind-syntax-p-helper ((term t) (used symbol-listp))
-    :returns (ok booleanp)
-    :short "Helper function for option-kind-syntax."
-    (b* ((used (symbol-list-fix used))
-         ((unless (consp term)) t)
-         ((unless (and (consp term) (consp (cdr term)))) nil)
-         ((list* first second rest) term)
-         ((if (member-equal first used))
-          (er hard? 'process=>option-kind-syntax-p-helper
-              "~p0 option is already defined in the hint.~%" first))
-         (first-ok
-          (case first
-            (:some (prod-kind-syntax-p second))
-            (:none (prod-kind-syntax-p second))
-            (t (er hard? 'process=>option-kind-syntax-p-helper
-                   "Smtlink-hint option-kind option doesn't include: ~p0.
-                       They are :some, and :none.~%"
-                   first)))))
-      (and first-ok
-           (option-kind-syntax-p-helper rest (cons first used))))
-    ///
-    (more-returns
-     (ok (implies (and ok (consp term) (symbol-listp used))
-                  (and (consp (cdr term))
-                       (not (member-equal (car term) used))
-                       (implies (equal (car term) :some)
-                                (prod-kind-syntax-p (cadr term)))
-                       (implies (equal (car term) :none)
-                                (prod-kind-syntax-p (cadr term)))))
-         :name definition-of-option-kind-syntax-p-helper
-         :hints (("Goal"
-                  :expand (option-kind-syntax-p-helper term used))))
-     (ok (implies (and ok (consp term) (symbol-listp used)
-                       (not (equal (car term) :some)))
-                  (equal (car term) :none))
-         :name option-of-option-kind-syntax-p-helper
-         :hints (("Goal"
-                  :expand (option-kind-syntax-p-helper term used)))))
-    (defthm monotonicity-of-option-kind-syntax-p-helper
-      (implies (and (subsetp used-1 used :test 'equal)
-                    (option-kind-syntax-p-helper term used))
-               (option-kind-syntax-p-helper term used-1))))
-
-  (defthm monotonicity-of-option-kind-syntax-p-helper-corollary
-    (implies (option-kind-syntax-p-helper term used)
-             (option-kind-syntax-p-helper term nil))
-    :hints (("Goal"
-             :in-theory (disable monotonicity-of-option-kind-syntax-p-helper)
-             :use ((:instance monotonicity-of-option-kind-syntax-p-helper
-                              (used used)
-                              (used-1 nil))))))
-
-  (define option-kind-syntax-p ((term t))
-    :returns (ok booleanp)
-    :short "Recoginizer for option-kind-syntax."
-    (option-kind-syntax-p-helper term nil)
-    ///
-    (more-returns
-     (ok (implies (and ok (consp term))
-                  (and (consp (cdr term))
-                       (implies (equal (car term) :some)
-                                (prod-kind-syntax-p (cadr term)))
-                       (implies (equal (car term) :none)
-                                (prod-kind-syntax-p (cadr term)))))
-         :name definition-of-option-kind-syntax-p
-         :hints (("Goal"
-                  :in-theory (disable definition-of-option-kind-syntax-p-helper)
-                  :use ((:instance
-                         definition-of-option-kind-syntax-p-helper
-                         (used nil))))))
-     (ok (implies (and ok (consp term)
-                       (not (equal (car term) :some)))
-                  (equal (car term) :none))
-         :name option-of-option-kind-syntax-p
-         :hints (("Goal"
-                  :in-theory (disable option-of-option-kind-syntax-p-helper)
-                  :use ((:instance
-                         option-of-option-kind-syntax-p-helper
-                         (used nil))))))
-     (ok (implies (and ok (consp term))
-                  (option-kind-syntax-p (cddr term)))
-         :hints (("Goal"
-                  :expand (option-kind-syntax-p-helper term nil)))
-         :name monotonicity-of-option-kind-syntax-p)))
-
-  (easy-fix option-kind-syntax nil)
-
-  ;; sum-kind
-  (define sum-kind-syntax-p-helper ((term t) (used symbol-listp))
-    :returns (ok booleanp)
-    :short "Helper function for sum-kind-syntax-p."
-    (b* ((used (symbol-list-fix used))
-         ((unless (consp term)) t)
-         ((unless (and (consp term) (consp (cdr term)))) nil)
-         ((list* first second rest) term)
-         ((if (member-equal first used))
-          (er hard? 'process=>sum-kind-syntax-p-helper
-              "~p0 option is already defined in the hint.~%" first))
-         (first-ok
-          (cond ((equal first :kind-fn) (symbolp second))
-                ((symbolp first) (prod-kind-syntax-p second))
-                (t (er hard? 'process=>sum-kind-syntax-p-helper
-                       "Smtlink-hint sum-kind option doesn't include: ~p0.
-                       They are :kind-fn, and tags.~%"
-                       first)))))
-      (and first-ok
-           (sum-kind-syntax-p-helper rest (cons first used))))
-    ///
-    (more-returns
-     (ok (implies (and ok (consp term) (symbol-listp used))
-                  (and (consp (cdr term))
-                       (not (member-equal (car term) used))
-                       (implies (equal (car term) :kind-fn)
-                                (symbolp (cadr term)))
-                       (implies (and (symbolp (car term))
-                                     (not (equal (car term) :kind-fn)))
-                                (prod-kind-syntax-p (cadr term)))))
-         :name definition-of-sum-kind-syntax-p-helper
-         :hints (("Goal"
-                  :expand (sum-kind-syntax-p-helper term used))))
-     (ok (implies (and ok (consp term) (symbol-listp used))
-                  (symbolp (car term)))
-         :name option-of-sum-kind-syntax-p-helper
-         :hints (("Goal"
-                  :expand (sum-kind-syntax-p-helper term used)))))
-    (defthm monotonicity-of-sum-kind-syntax-p-helper
-      (implies (and (subsetp used-1 used :test 'equal)
-                    (sum-kind-syntax-p-helper term used))
-               (sum-kind-syntax-p-helper term used-1))))
-
-  (defthm monotonicity-of-sum-kind-syntax-p-helper-corollary
-    (implies (sum-kind-syntax-p-helper term used)
-             (sum-kind-syntax-p-helper term nil))
-    :hints (("Goal"
-             :in-theory (disable monotonicity-of-sum-kind-syntax-p-helper)
-             :use ((:instance monotonicity-of-sum-kind-syntax-p-helper
-                              (used used)
-                              (used-1 nil))))))
-
-  (define sum-kind-syntax-p ((term t))
-    :returns (ok booleanp)
-    :short "Recognizer for sum-kind-syntax."
-    (sum-kind-syntax-p-helper term nil)
-    ///
-    (more-returns
-     (ok (implies (and ok (consp term))
-                  (and (consp (cdr term))
-                       (implies (equal (car term) :kind-fn)
-                                (symbolp (cadr term)))
-                       (implies (and (symbolp (car term))
-                                     (not (equal (car term) :kind-fn)))
-                                (prod-kind-syntax-p (cadr term)))))
-         :name definition-of-sum-kind-syntax-p
-         :hints (("Goal"
-                  :in-theory (disable definition-of-sum-kind-syntax-p-helper)
-                  :use ((:instance
-                         definition-of-sum-kind-syntax-p-helper
-                         (used nil))))))
-     (ok (implies (and ok (consp term))
-                  (symbolp (car term)))
-         :name option-of-sum-kind-syntax-p
-         :hints (("Goal"
-                  :in-theory (disable option-of-sum-kind-syntax-p-helper)
-                  :use ((:instance
-                         option-of-sum-kind-syntax-p-helper
-                         (used nil))))))
-     (ok (implies (and ok (consp term))
-                  (sum-kind-syntax-p (cddr term)))
-         :hints (("Goal"
-                  :expand (sum-kind-syntax-p-helper term nil)))
-         :name monotonicity-of-sum-kind-syntax-p)))
-
-  (easy-fix sum-kind-syntax nil)
-
-  ;; kind syntax
-  (define kind-syntax-p ((term t))
-    :returns (ok booleanp)
-    :short "Recognizer for kind-syntax."
-    (b* (((unless (consp term)) nil)
-         ((cons kind options) term))
-      (case kind
-        (:abstract (abstract-kind-syntax-p options))
-        (:array (array-kind-syntax-p options))
-        (:prod (prod-kind-syntax-p options))
-        (:sum (sum-kind-syntax-p options))
-        (:list (list-kind-syntax-p options))
-        (:option (option-kind-syntax-p options))
-        (t (er hard? 'process=>kind-syntax-p
-               "Smtlink-hint kind-syntax option doesn't include: ~p0.
-                       They are :abstract, :list, :array, :prod, :option, and
-                       :sum.~%" kind))))
-    ///
-    (more-returns
-     (ok
-      (implies ok
-               (and (consp term)
-                    (implies (equal (car term) :abstract)
-                             (abstract-kind-syntax-p (cdr term)))
-                    (implies (equal (car term) :array)
-                             (array-kind-syntax-p (cdr term)))
-                    (implies (equal (car term) :prod)
-                             (prod-kind-syntax-p (cdr term)))
-                    (implies (equal (car term) :sum)
-                             (sum-kind-syntax-p (cdr term)))
-                    (implies (equal (car term) :list)
-                             (list-kind-syntax-p (cdr term)))
-                    (implies (equal (car term) :option)
-                             (option-kind-syntax-p (cdr term)))))
-      :name definition-of-kind-syntax-p)
-     (ok (implies (and ok
-                       (not (equal (car term) :abstract))
-                       (not (equal (car term) :array))
-                       (not (equal (car term) :prod))
-                       (not (equal (car term) :list))
-                       (not (equal (car term) :option)))
-                  (equal (car term) :sum))
-         :name option-of-kind-syntax-p))
-    )
-
-  (easy-fix kind-syntax '(:abstract))
   )
 
 (defsection type-option-syntax
@@ -1019,36 +276,27 @@
               "~p0 option is already defined in the hint.~%" first))
          (first-ok
           (case first
-            (:recognizer (symbolp second))
-            (:fixer (symbolp second))
-            (:fixer-when-recognizer-thm (symbolp second))
-            (:kind (kind-syntax-p second))
+            (:functions (function-list-syntax-p second))
+            (:subtypes (symbol-listp second))
             (t (er hard? 'process=>type-option-syntax-p-helper
                    "Smtlink-hint type option doesn't include: ~p0.
-                       They are :recognizer, :fixer,
-                       :fixer-when-recognizer-thm, and :kind.~%" first)))))
+                       They are :functions, and :subtypes.~%" first)))))
       (and first-ok
            (type-option-syntax-p-helper rest (cons first used))))
     ///
     (more-returns
      (ok (implies (and ok (consp term) (symbol-listp used))
                   (and (consp (cdr term))
-                       (implies (equal (car term) :recognizer)
-                                (symbolp (cadr term)))
-                       (implies (equal (car term) :fixer)
-                                (symbolp (cadr term)))
-                       (implies (equal (car term) :fixer-when-recognizer-thm)
-                                (symbolp (cadr term)))
-                       (implies (equal (car term) :kind)
-                                (kind-syntax-p (cadr term)))))
+                       (implies (equal (car term) :functions)
+                                (function-list-syntax-p (cadr term)))
+                       (implies (equal (car term) :subtypes)
+                                (symbol-listp (cadr term)))))
          :hints (("Goal"
                   :expand (type-option-syntax-p-helper term used)))
          :name definition-of-type-option-syntax-p-helper)
      (ok (implies (and (and ok (consp term) (symbol-listp used))
-                       (not (equal (car term) :recognizer))
-                       (not (equal (car term) :fixer))
-                       (not (equal (car term) :fixer-when-recognizer-thm)))
-                  (equal (car term) :kind))
+                       (not (equal (car term) :functions)))
+                  (equal (car term) :subtypes))
          :hints (("Goal"
                   :expand (type-option-syntax-p-helper term used)))
          :name option-of-type-option-syntax-p-helper))
@@ -1074,20 +322,14 @@
     (more-returns
      (ok (implies (and ok (consp term))
                   (and (consp (cdr term))
-                       (implies (equal (car term) :recognizer)
-                                (symbolp (cadr term)))
-                       (implies (equal (car term) :fixer)
-                                (symbolp (cadr term)))
-                       (implies (equal (car term) :fixer-when-recognizer-thm)
-                                (symbolp (cadr term)))
-                       (implies (equal (car term) :kind)
-                                (kind-syntax-p (cadr term)))))
+                       (implies (equal (car term) :functions)
+                                (function-list-syntax-p (cadr term)))
+                       (implies (equal (car term) :subtypes)
+                                (symbol-listp (cadr term)))))
          :name definition-of-type-option-syntax-p)
      (ok (implies (and (and ok (consp term))
-                       (not (equal (car term) :recognizer))
-                       (not (equal (car term) :fixer))
-                       (not (equal (car term) :fixer-when-recognizer-thm)))
-                  (equal (car term) :kind))
+                       (not (equal (car term) :functions)))
+                  (equal (car term) :subtypes))
          :name option-of-type-option-syntax-p)
      (ok (implies (and ok (consp term))
                   (type-option-syntax-p (cddr term)))
@@ -1112,9 +354,9 @@
 
   (easy-fix type-syntax nil)
 
-  (deflist type-lst-syntax
+  (deflist type-list-syntax
     :elt-type type-syntax-p
-    :pred type-lst-syntax-p
+    :pred type-list-syntax-p
     :true-listp t)
   )
 
@@ -1152,23 +394,21 @@
               "~p0 option is already defined in the hint.~%" first))
          (first-ok
           (case first
-            (:functions (function-lst-syntax-p second))
-            (:types (type-lst-syntax-p second))
-            (:hypotheses (hypothesis-lst-syntax-p second))
-            (:rm-file (booleanp second))
+            (:functions (function-list-syntax-p second))
+            (:hypotheses (hypothesis-list-syntax-p second))
+            (:types (type-list-syntax-p second))
+            (:int-to-ratp (int-to-rat-syntax-p second))
+            (:under-inductionp (booleanp second))
             (:smt-dir (stringp second))
             (:smt-fname (stringp second))
-            (:int-to-rat (int-to-rat-syntax-p second))
-            (:use-uninterpreted (booleanp second))
-            (:under-induct (symbolp second))
+            (:rm-file (booleanp second))
             (:global-hint (symbolp second))
-            (:custom-p (booleanp second))
-            (:wrld-fn-len (natp second))
+            (:customp (booleanp second))
             (t (er hard? 'process=>smtlink-hint-syntax-p-helper
-                   "Smtlink-hint option doesn't include: ~p0.
-                       They are :functions, :types, :hypotheses, :rm-file,
-                       :smt-dir, :smt-fname, :int-to-rat, :use-uninterpreted,
-                       :under-induct, and :global-hint.~%" first)))))
+                   "Smtlink-hint option doesn't include: ~p0. ~
+                       They are :functions, :hypotheses, :types, :int-to-ratp, ~
+                       :under-inductionp, :smt-dir, :smt-fname, :rm-file, ~
+                       :smt-solver-params, :customp.~%" first)))))
       (and first-ok
            (smtlink-hint-syntax-p-helper rest (cons first used))))
     ///
@@ -1176,45 +416,39 @@
      (ok (implies (and ok (consp term) (symbol-listp used))
                   (and (consp (cdr term))
                        (implies (equal (car term) :functions)
-                                (function-lst-syntax-p (cadr term)))
-                       (implies (equal (car term) :types)
-                                (type-lst-syntax-p (cadr term)))
+                                (function-list-syntax-p (cadr term)))
                        (implies (equal (car term) :hypotheses)
-                                (hypothesis-lst-syntax-p (cadr term)))
-                       (implies (equal (car term) :rm-file)
+                                (hypothesis-list-syntax-p (cadr term)))
+                       (implies (equal (car term) :types)
+                                (type-list-syntax-p (cadr term)))
+                       (implies (equal (car term) :int-to-ratp)
+                                (int-to-rat-syntax-p (cadr term)))
+                       (implies (equal (car term) :under-inductionp)
                                 (booleanp (cadr term)))
                        (implies (equal (car term) :smt-dir)
                                 (stringp (cadr term)))
                        (implies (equal (car term) :smt-fname)
                                 (stringp (cadr term)))
-                       (implies (equal (car term) :int-to-rat)
-                                (int-to-rat-syntax-p (cadr term)))
-                       (implies (equal (car term) :use-uninterpreted)
+                       (implies (equal (car term) :rm-file)
                                 (booleanp (cadr term)))
-                       (implies (equal (car term) :under-induct)
-                                (symbolp (cadr term)))
                        (implies (equal (car term) :global-hint)
                                 (symbolp (cadr term)))
-                       (implies (equal (car term) :custom-p)
-                                (booleanp (cadr term)))
-                       (implies (equal (car term) :wrld-fn-len)
-                                (natp (cadr term)))))
+                       (implies (equal (car term) :customp)
+                                (booleanp (cadr term)))))
          :hints (("Goal"
                   :expand (smtlink-hint-syntax-p-helper term used)))
          :name definition-of-smtlink-hint-syntax-p-helper)
      (ok (implies (and (and ok (consp term))
                        (not (equal (car term) :functions))
-                       (not (equal (car term) :types))
                        (not (equal (car term) :hypotheses))
-                       (not (equal (car term) :rm-file))
+                       (not (equal (car term) :types))
+                       (not (equal (car term) :int-to-ratp))
+                       (not (equal (car term) :under-inductionp))
                        (not (equal (car term) :smt-dir))
                        (not (equal (car term) :smt-fname))
-                       (not (equal (car term) :int-to-rat))
-                       (not (equal (car term) :use-uninterpreted))
-                       (not (equal (car term) :under-induct))
-                       (not (equal (car term) :global-hint))
-                       (not (equal (car term) :custom-p)))
-                  (equal (car term) :wrld-fn-len))
+                       (not (equal (car term) :rm-file))
+                       (not (equal (car term) :global-hint)))
+                  (equal (car term) :customp))
          :hints (("Goal"
                   :expand (smtlink-hint-syntax-p-helper term used)))
          :name option-of-smtlink-hint-syntax-p-helper))
@@ -1241,43 +475,37 @@
      (ok (implies (and ok (consp term))
                   (and (consp (cdr term))
                        (implies (equal (car term) :functions)
-                                (function-lst-syntax-p (cadr term)))
-                       (implies (equal (car term) :types)
-                                (type-lst-syntax-p (cadr term)))
+                                (function-list-syntax-p (cadr term)))
                        (implies (equal (car term) :hypotheses)
-                                (hypothesis-lst-syntax-p (cadr term)))
-                       (implies (equal (car term) :rm-file)
+                                (hypothesis-list-syntax-p (cadr term)))
+                       (implies (equal (car term) :types)
+                                (type-list-syntax-p (cadr term)))
+                       (implies (equal (car term) :int-to-ratp)
+                                (int-to-rat-syntax-p (cadr term)))
+                       (implies (equal (car term) :under-inductionp)
                                 (booleanp (cadr term)))
                        (implies (equal (car term) :smt-dir)
                                 (stringp (cadr term)))
                        (implies (equal (car term) :smt-fname)
                                 (stringp (cadr term)))
-                       (implies (equal (car term) :int-to-rat)
-                                (int-to-rat-syntax-p (cadr term)))
-                       (implies (equal (car term) :use-uninterpreted)
+                       (implies (equal (car term) :rm-file)
                                 (booleanp (cadr term)))
-                       (implies (equal (car term) :under-induct)
-                                (symbolp (cadr term)))
                        (implies (equal (car term) :global-hint)
                                 (symbolp (cadr term)))
-                       (implies (equal (car term) :custom-p)
-                                (booleanp (cadr term)))
-                       (implies (equal (car term) :wrld-fn-len)
-                                (natp (cadr term)))))
+                       (implies (equal (car term) :customp)
+                                (booleanp (cadr term)))))
          :name definition-of-smtlink-hint-syntax-p)
      (ok (implies (and (and ok (consp term))
                        (not (equal (car term) :functions))
-                       (not (equal (car term) :types))
                        (not (equal (car term) :hypotheses))
-                       (not (equal (car term) :rm-file))
+                       (not (equal (car term) :types))
+                       (not (equal (car term) :int-to-ratp))
+                       (not (equal (car term) :under-inductionp))
                        (not (equal (car term) :smt-dir))
                        (not (equal (car term) :smt-fname))
-                       (not (equal (car term) :int-to-rat))
-                       (not (equal (car term) :use-uninterpreted))
-                       (not (equal (car term) :under-induct))
-                       (not (equal (car term) :global-hint))
-                       (not (equal (car term) :custom-p)))
-                  (equal (car term) :wrld-fn-len))
+                       (not (equal (car term) :rm-file))
+                       (not (equal (car term) :global-hint)))
+                  (equal (car term) :customp))
          :name option-of-smtlink-hint-syntax-p)
      (ok (implies (and ok (consp term))
                   (smtlink-hint-syntax-p (cddr term)))
@@ -1303,45 +531,24 @@
                            acl2::true-listp-of-car-when-true-list-listp
                            acl2::pseudo-term-listp-cdr)))
 
-  (define construct-argument-list ((content argument-lst-syntax-p))
-    :returns (decls decl-list-p)
-    :short "Translate arguments into smtlink-hint structure."
-    :measure (len content)
-    :guard-hints (("Goal" :in-theory (e/d (argument-syntax-p
-                                           smt-typep)
-                                          ())))
-    (b* ((content (argument-lst-syntax-fix content))
-         ((unless (consp content)) nil)
-         ((cons first rest) content)
-         ((list argname type & thm-name) first)
-         (new-formal (make-decl :name argname
-                                :type (make-hint-pair :thm `(,type ,argname)
-                                                      :name thm-name))))
-      (cons new-formal (construct-argument-list rest))))
+(define construct-return ((return return-syntax-p))
+  :returns (smt-return smt-return-p)
+  :guard-hints (("Goal" :in-theory (enable return-syntax-p)))
+  (b* ((return (return-syntax-fix return)))
+    (make-smt-return :var (car return) :thm (caddr return))))
 
-  (define construct-hypothesis ((content hypothesis-syntax-p))
-    :returns (hypo hint-pair-p)
-    :short "Translate one hypothesis into smtlink-hint structure."
-    :guard-hints (("Goal" :in-theory (enable hypothesis-syntax-p)))
-    (b* ((content (hypothesis-syntax-fix content))
-         ((list thm tag hints/thm-name) content)
-         (new-hypo (if (equal tag :name)
-                       (make-hint-pair :thm thm :name hints/thm-name)
-                     (make-hint-pair :thm thm :hints hints/thm-name))))
-      new-hypo))
+(define construct-return-list ((return-lst return-list-syntax-p))
+  :returns (smt-return-lst smt-return-list-p)
+  :hints (("Goal" :in-theory (enable return-list-syntax-fix)))
+  :guard-hints (("Goal" :in-theory (enable return-list-syntax-p)))
+  :measure (len return-lst)
+  (b* ((return-lst (return-list-syntax-fix return-lst))
+       ((unless (consp return-lst)) nil)
+       ((cons return-hd return-tl) return-lst))
+    (cons (construct-return return-hd) (construct-return-list return-tl))))
 
-  (define construct-hypothesis-list ((content hypothesis-lst-syntax-p))
-    :returns (hypos hint-pair-list-p)
-    :short "Translate a list of hypotheses into smtlink-hint structure."
-    :measure (len content)
-    (b* ((content (hypothesis-lst-syntax-fix content))
-         ((unless (consp content)) nil)
-         ((cons first rest) content)
-         (new-hypo (construct-hypothesis first)))
-      (cons new-hypo (construct-hypothesis-list rest))))
-
-  (define construct-function-option-lst ((fun-opt-lst function-option-syntax-p)
-                                        (smt-func smt-function-p))
+(define construct-function-option-lst ((fun-opt-lst function-option-syntax-p)
+                                       (smt-func smt-function-p))
     :returns (func smt-function-p)
     :short "Add option information into func."
     :measure (len fun-opt-lst)
@@ -1352,19 +559,13 @@
          ((list* option content rest) fun-opt-lst)
          (new-smt-func
           (case option
-            (:expansion-depth (change-smt-function smt-func :expansion-depth content))
-            (:formals (change-smt-function
-                       smt-func
-                       :formals (construct-argument-list content)))
-            (:returns (change-smt-function
-                       smt-func
-                       :returns (construct-argument-list content)))
-            (:guard (change-smt-function
-                     smt-func
-                     :guard (construct-hypothesis content)))
-            (:more-returns (change-smt-function
-                            smt-func
-                            :more-returns (construct-hypothesis-list content))))))
+            (:formals (change-smt-function smt-func :formals content))
+            (:return (change-smt-function smt-func :returns
+                                          (construct-return-list content)))
+            (:uninterpreted-hints (change-smt-function smt-func
+                                                       :uninterpreted-hints content))
+            (:replace (change-smt-function smt-func :replace-thm content))
+            (:depth (change-smt-function smt-func :depth content)))))
       (construct-function-option-lst rest new-smt-func)))
 
   (define construct-function ((func function-syntax-p))
@@ -1376,18 +577,18 @@
       (construct-function-option-lst fun-opt-lst
                                      (make-smt-function :name name))))
 
-  (define merge-functions ((content function-lst-syntax-p)
+  (define merge-functions ((content function-list-syntax-p)
                            (hint smtlink-hint-p))
     :returns (new-hint smtlink-hint-p)
     :short "Merging function hints into smt-hint."
     :measure (len content)
-    :hints (("Goal" :in-theory (enable function-lst-syntax-fix)))
-    :guard-hints (("Goal" :in-theory (enable function-lst-syntax-fix
-                                             function-lst-syntax-p
+    :hints (("Goal" :in-theory (enable function-list-syntax-fix)))
+    :guard-hints (("Goal" :in-theory (enable function-list-syntax-fix
+                                             function-list-syntax-p
                                              function-syntax-p
                                              function-syntax-fix)))
     (b* ((hint (smtlink-hint-fix hint))
-         (content (function-lst-syntax-fix content))
+         (content (function-list-syntax-fix content))
          ((unless (consp content)) hint)
          ((cons first rest) content)
          ((smtlink-hint h) hint)
@@ -1396,258 +597,45 @@
       (merge-functions rest new-hint)))
 
 ;; construct types
-(define construct-type-thm-options ((content type-thm-syntax-p)
-                                    (tt type-thm-p))
-  :returns (new-tt type-thm-p)
-  :measure (len content)
-  :hints (("Goal" :in-theory (enable type-thm-syntax-fix)))
-  (b* ((content (type-thm-syntax-fix content))
-       (tt (type-thm-fix tt))
-       ((unless (consp content)) tt)
-       ((list* first second rest) content)
-       (new-tt
-        (case first
-          (:name (change-type-thm tt :name second))
-          (:hints (change-type-thm tt :hints second)))))
-    (construct-type-thm-options rest new-tt)))
+(define construct-type-functions ((func-lst function-list-syntax-p))
+  :returns (new-func-lst smt-function-list-p)
+  :measure (len func-lst)
+  (b* ((func-lst (function-list-syntax-fix func-lst))
+       ((unless (consp func-lst)) nil)
+       ((cons func-hd func-tl) func-lst))
+    (cons (construct-function func-hd) (construct-type-functions func-tl))))
 
-(define construct-type-thm ((content type-thm-syntax-p))
-  :returns (new-tt type-thm-p)
-  (construct-type-thm-options content (make-type-thm)))
-
-(define construct-type-function-option-list ((content type-function-option-syntax-p)
-                                             (tf type-function-p))
-  :returns (new-tf type-function-p)
-  :measure (len content)
-  :hints (("Goal" :in-theory (enable type-function-option-syntax-fix)))
-  (b* ((content (type-function-option-syntax-fix content))
-       (tf (type-function-fix tf))
-       ((unless (consp content)) tf)
-       ((list* first second rest) content)
-       (new-tf
-        (case first
-          (:return-type (change-type-function tf :return-type second))
-          (:type-thm
-           (change-type-function tf
-                                 :type-of-function-thm
-                                 (construct-type-thm second)))
-          (:destructor-thm
-           (change-type-function tf
-                                 :destructor-of-constructor-thm
-                                 (construct-type-thm second))))))
-    (construct-type-function-option-list rest new-tf)))
-
-(define construct-type-function ((content type-function-syntax-p)
-                                 (acc symbol-listp))
-  :returns (mv (new-tf type-function-p)
-               (new-acc symbol-listp
-                        :hints (("Goal"
-                                 :in-theory (enable type-function-syntax-fix
-                                                    type-function-syntax-p)))))
-  :guard-hints (("Goal"
-                 :in-theory (enable type-function-syntax-p)))
-  (b* ((content (type-function-syntax-fix content))
-       (acc (symbol-list-fix acc))
-       ((cons name options) content)
-       ((if (member-equal name acc))
-        (mv (make-type-function)
-            (er hard? 'process=>construct-type-function
-                "Redefinition of function ~p0" name))))
-    (mv (construct-type-function-option-list
-         options
-         (make-type-function :name name))
-        (cons name acc))))
-
-(define construct-type-function-list ((content type-function-list-syntax-p)
-                                      (acc symbol-listp))
-  :returns (mv (new-lst type-function-list-p)
-               (new-acc symbol-listp))
-  :measure (len content)
-  :guard-hints (("Goal"
-                 :in-theory (enable type-function-syntax-p)))
-  (b* ((content (type-function-list-syntax-fix content))
-       (acc (symbol-list-fix acc))
-       ((unless (consp content)) (mv nil acc))
-       ((cons first rest) content)
-       ((mv first-fn new-acc)
-        (construct-type-function first acc))
-       ((mv rest-fn fin-acc)
-        (construct-type-function-list rest new-acc)))
-    (mv (cons first-fn rest-fn)
-        fin-acc)))
-
-  (define construct-array-kind ((content array-kind-syntax-p)
-                                (smt-type-array smt-type-p))
-    :returns (new-array smt-type-p)
-    :guard (equal (smt-type-kind smt-type-array) :array)
-    :irrelevant-formals-ok t
-    :ignore-ok t
-    (smt-type-fix smt-type-array))
-
-  (define construct-prod-kind ((content prod-kind-syntax-p)
-                               (prod prod-p)
-                               (acc symbol-listp))
-    :returns (mv (new-prod prod-p)
-                 (new-acc symbol-listp))
-    :measure (len content)
-    :hints (("Goal"
-             :in-theory (enable prod-kind-syntax-fix)))
-    (b* ((content (prod-kind-syntax-fix content))
-         (acc (symbol-list-fix acc))
-         (prod (prod-fix prod))
-         ((unless (consp content)) (mv prod acc))
-         ((list* first second rest) content)
-         ((mv new-prod new-acc)
-          (case first
-            (:constructor
-             (b* (((mv constructor-fn new-acc)
-                   (construct-type-function second acc)))
-               (mv (change-prod prod :constructor constructor-fn)
-                   new-acc)))
-            (:destructors
-             (b* (((mv destructor-fns new-acc)
-                   (construct-type-function-list second acc)))
-               (mv (change-prod prod :destructors destructor-fns)
-                   new-acc)))
-            (t (mv prod acc)))))
-      (construct-prod-kind rest new-prod new-acc)))
-
-;; difference prods can have the functions of the same name!!!
-  (define construct-sum-kind ((content sum-kind-syntax-p)
-                              (smt-type-sum smt-type-p)
-                              (acc symbol-listp))
-    :returns (mv (new-sum smt-type-p)
-                 (new-acc symbol-listp))
-    :guard (equal (smt-type-kind smt-type-sum) :sum)
-    :measure (len content)
-    :hints (("Goal"
-             :in-theory (enable sum-kind-syntax-fix)))
-    (b* ((content (sum-kind-syntax-fix content))
-         (acc (symbol-list-fix acc))
-         (smt-type-sum (smt-type-fix smt-type-sum))
-         ((unless (consp content)) (mv smt-type-sum acc))
-         ((list* first second rest) content)
-         ((if (member-equal first acc))
-          (prog2$ (er hard? 'process=>construct-sum-kind
-                      "Redefining kind ~q0" first)
-                  (mv (make-smt-type-abstract) nil)))
-         ((smt-type-sum s) smt-type-sum)
-         ((mv new-type new-acc)
-          (case first
-            (:kind-fn (mv (change-smt-type-sum s :kind-fn second)
-                          acc))
-            (t
-             (b* (((mv new-prod &)
-                   (construct-prod-kind second (make-prod :kind first) nil)))
-               (mv (change-smt-type-sum s :prods (cons new-prod s.prods))
-                   (cons first acc)))))))
-      (construct-sum-kind rest new-type new-acc))
-    )
-
-(define construct-list-kind ((content list-kind-syntax-p)
-                             (smt-type-list smt-type-p))
-  :returns (new-list smt-type-p)
-  :guard (equal (smt-type-kind smt-type-list) :sum)
-  :measure (len content)
-  :hints (("Goal" :in-theory (enable list-kind-syntax-fix)))
-  (b* ((content (list-kind-syntax-fix content))
-       (smt-type-list (smt-type-fix smt-type-list))
-       ((unless (consp content)) smt-type-list)
-       ((list* first second rest) content)
-       ((smt-type-sum s) smt-type-list)
-       (new-type
-        (case first
-          (:cons (b* (((mv new-prod &)
-                       (construct-prod-kind second (make-prod :kind first) nil)))
-                   (change-smt-type-sum s :prods (cons new-prod s.prods))))
-          (:nil-kind (b* (((mv new-prod &)
-                           (construct-prod-kind second (make-prod :kind first) nil)))
-                       (change-smt-type-sum s :prods (cons new-prod s.prods)))))))
-    (construct-list-kind rest new-type))
-  )
-
-(define construct-option-kind ((content option-kind-syntax-p)
-                               (smt-type-option smt-type-p))
-  :returns (new-option smt-type-p)
-  :guard (equal (smt-type-kind smt-type-option) :sum)
-  :measure (len content)
-  :hints (("Goal" :in-theory (enable option-kind-syntax-fix)))
-  (b* ((content (option-kind-syntax-fix content))
-       (smt-type-option (smt-type-fix smt-type-option))
-       ((unless (consp content)) smt-type-option)
-       ((list* first second rest) content)
-       ((smt-type-sum s) smt-type-option)
-       (new-type
-        (case first
-          (:some (b* (((mv new-prod &)
-                       (construct-prod-kind second (make-prod :kind first) nil)))
-                   (change-smt-type-sum s :prods (cons new-prod s.prods))))
-          (:none (b* (((mv new-prod &)
-                       (construct-prod-kind second (make-prod :kind first) nil)))
-                   (change-smt-type-sum s :prods (cons new-prod s.prods)))))))
-    (construct-option-kind rest new-type)))
-
-  (define construct-kind ((content kind-syntax-p))
-    :returns (new-kind smt-type-p)
-    (b* ((content (kind-syntax-fix content))
-         ((cons kind options) content))
-      (case kind
-       (:abstract (make-smt-type-abstract))
-       (:array
-        (construct-array-kind options (make-smt-type-array)))
-       (:prod
-        (b* (((mv new-prod &)
-              (construct-prod-kind options (make-prod) nil)))
-          (make-smt-type-sum :kind-fn nil
-                             :prods (list new-prod))))
-       (:sum
-        (b* (((mv new-type &)
-              (construct-sum-kind options (make-smt-type-sum) nil)))
-          new-type))
-       (:list
-        (construct-list-kind options (make-smt-type-sum)))
-       (:option
-        (construct-option-kind options (make-smt-type-sum))))))
-
-  (define construct-type-option-lst ((type-opt-lst type-option-syntax-p)
-                                     (smt-type smt-fixtype-p))
-    :returns (new-type smt-fixtype-p)
-    :short "Add option information into smt-type."
+(define construct-type-option-lst ((type-opt-lst type-option-syntax-p)
+                                   (smt-type smt-type-p))
+    :returns (smt-type smt-type-p)
     :measure (len type-opt-lst)
     :hints (("Goal" :in-theory (enable type-option-syntax-fix)))
     (b* ((type-opt-lst (type-option-syntax-fix type-opt-lst))
-         (smt-type (smt-fixtype-fix smt-type))
-         ((unless (and (consp type-opt-lst) (consp (cdr type-opt-lst)))) smt-type)
+         (smt-type (smt-type-fix smt-type))
+         ((unless (consp type-opt-lst)) smt-type)
          ((list* option content rest) type-opt-lst)
          (new-smt-type
           (case option
-            (:recognizer (change-smt-fixtype smt-type :recognizer content))
-            (:fixer (change-smt-fixtype smt-type :fixer content))
-            (:fixer-when-recognizer-thm
-             (change-smt-fixtype
-              smt-type :fixer-when-recognizer-thm
-              (make-type-thm :name content)))
-            (:kind (change-smt-fixtype
-                    smt-type
-                    :kind (construct-kind content))))))
+            (:functions
+             (change-smt-type smt-type
+                              :functions (construct-type-functions content)))
+            (:subtypes (change-smt-type smt-type :subtypes content)))))
       (construct-type-option-lst rest new-smt-type)))
 
   (define construct-type ((type type-syntax-p))
-    :returns (new-type smt-fixtype-p)
-    :guard-hints (("Goal"
-                   :in-theory (enable type-syntax-p)))
+    :returns (new-type smt-type-p)
+    :guard-hints (("Goal" :in-theory (enable type-syntax-fix type-syntax-p)))
     (b* ((type (type-syntax-fix type))
          ((cons name type-opt-lst) type))
-      (construct-type-option-lst type-opt-lst
-                                (make-smt-fixtype :name name))))
+      (construct-type-option-lst type-opt-lst (make-smt-type :recognizer name))))
 
-  (define merge-types ((content type-lst-syntax-p)
+  (define merge-types ((content type-list-syntax-p)
                        (hint smtlink-hint-p))
     :returns (new-hint smtlink-hint-p)
     :measure (len content)
     :short "Merging type hints into smt-hint."
     (b* ((hint (smtlink-hint-fix hint))
-         (content (type-lst-syntax-fix content))
+         (content (type-list-syntax-fix content))
          ((unless (consp content)) hint)
          ((cons first rest) content)
          ((smtlink-hint h) hint)
@@ -1655,12 +643,23 @@
          (new-hint (change-smtlink-hint h :types new-type-lst)))
       (merge-types rest new-hint)))
 
-  (define merge-hypotheses ((content hypothesis-lst-syntax-p)
+(define construct-hypothesis ((hypo hypothesis-syntax-p))
+  :returns (smt-hypo smt-hypo-p)
+  :guard-hints (("Goal" :in-theory (enable hypothesis-syntax-p
+                                           subst-syntax-p)))
+  (b* ((hypo (hypothesis-syntax-fix hypo)))
+    (case-match hypo
+      ((':instance thm subst)
+       (make-smt-hypo :thm thm :subst (pairlis$ (strip-cars subst)
+                                                (strip-cadrs subst))))
+      (& (make-smt-hypo :thm (cadr hypo))))))
+
+(define merge-hypotheses ((content hypothesis-list-syntax-p)
                             (hint smtlink-hint-p))
     :returns (new-hint smtlink-hint-p)
     :short "Merging type hints into smt-hint."
     :measure (len content)
-    (b* ((content (hypothesis-lst-syntax-fix content))
+    (b* ((content (hypothesis-list-syntax-fix content))
          (hint (smtlink-hint-fix hint))
          ((smtlink-hint h) hint)
          ((unless (consp content)) h)
@@ -1702,7 +701,7 @@
   (define set-int-to-rat ((content int-to-rat-syntax-p)
                           (hint smtlink-hint-p))
     :returns (new-hint smtlink-hint-p)
-    :short "Set :int-to-rat based on user hint."
+    :short "Set :int-to-ratp based on user hint."
     :guard-hints (("Goal"
                    :in-theory (disable definition-of-int-to-rat-syntax-p)
                    :use ((:instance definition-of-int-to-rat-syntax-p
@@ -1713,7 +712,7 @@
           (if (booleanp content)
               (make-int-to-rat-switch :okp content)
             (make-int-to-rat-symbol-list :lst content)))
-         (new-hint (change-smtlink-hint hint :int-to-rat new-int-to-rat)))
+         (new-hint (change-smtlink-hint hint :int-to-ratp new-int-to-rat)))
       new-hint))
 
   (define set-smt-cnf ((content booleanp)
@@ -1727,20 +726,12 @@
          (new-hint (change-smtlink-hint hint :configurations new-cnf)))
       new-hint))
 
-  (define set-use-uninterpreted ((content booleanp)
-                                 (hint smtlink-hint-p))
-    :returns (new-hint smtlink-hint-p)
-    :short "Set :use-uninterpreted"
-    (b* ((hint (smtlink-hint-fix hint))
-         (new-hint (change-smtlink-hint hint :use-uninterpreted content)))
-      new-hint))
-
-  (define set-under-induct ((content symbolp)
+  (define set-under-induct ((content booleanp)
                             (hint smtlink-hint-p))
     :returns (new-hint smtlink-hint-p)
     :short "Set :under-induct"
     (b* ((hint (smtlink-hint-fix hint))
-         (new-hint (change-smtlink-hint hint :under-induct content)))
+         (new-hint (change-smtlink-hint hint :under-inductionp content)))
       new-hint))
 
   (define set-global-hint ((content symbolp)
@@ -1750,14 +741,6 @@
     (b* ((hint (smtlink-hint-fix hint))
          (new-hint (change-smtlink-hint hint :global-hint content)))
       new-hint))
-
-(define set-wrld-len ((content natp)
-                      (hint smtlink-hint-p))
-  :returns (new-hint smtlink-hint-p)
-  :short "Set :global-hint"
-  (b* ((hint (smtlink-hint-fix hint))
-       (new-hint (change-smtlink-hint hint :wrld-fn-len content)))
-    new-hint))
 
   (define combine-hints ((user-hint smtlink-hint-syntax-p)
                          (hint smtlink-hint-p))
@@ -1771,17 +754,15 @@
          ((list* option second rest) user-hint)
          (new-hint (case option
                      (:functions (merge-functions second hint))
-                     (:types (merge-types second hint))
                      (:hypotheses (merge-hypotheses second hint))
+                     (:types (merge-types second hint))
+                     (:int-to-ratp (set-int-to-rat second hint))
+                     (:under-inductionp (set-under-induct second hint))
+                     (:smt-fname (set-fname second hint))
                      (:rm-file (set-rm-file second hint))
                      (:smt-dir (set-smt-dir second hint))
-                     (:smt-fname (set-fname second hint))
-                     (:int-to-rat (set-int-to-rat second hint))
-                     (:use-uninterpreted (set-use-uninterpreted second hint))
-                     (:under-induct (set-under-induct second hint))
                      (:global-hint (set-global-hint second hint))
-                     (:custom-p (set-smt-cnf second hint))
-                     (:wrld-fn-len (set-wrld-len second hint)))))
+                     (:customp (set-smt-cnf second hint)))))
       (combine-hints rest new-hint)))
 
 (define find-global-hint-helper ((user-hint smtlink-hint-syntax-p))
@@ -1824,7 +805,6 @@
 
   (define process-hint ((cl pseudo-term-listp) (user-hint t) state)
     :returns (subgoal-lst pseudo-term-list-listp)
-    :guard-debug t
     (b* ((cl (pseudo-term-list-fix cl))
          ((unless (smtlink-hint-syntax-p user-hint))
           (prog2$ (cw "User provided Smtlink hint can't be applied because of ~
@@ -1837,8 +817,7 @@
           (prog2$ (cw "The hint ~p0 from state is not smtlink-hint-p:
     ~p1~%Therefore proceed without Smtlink...~%" the-hint user-hint)
                   (list cl)))
-         (combined-hint-w/o-info (combine-hints user-hint the-hint))
-         (combined-hint (add-fixtype-info combined-hint-w/o-info))
+         (combined-hint (combine-hints user-hint the-hint))
          ;; (- (cw "combined-hint: ~q0" combined-hint))
          (next-cp (cdr (assoc-equal 'process-hint *SMT-architecture*)))
          ((if (null next-cp)) (list cl))
@@ -1852,142 +831,6 @@
     (b* ((expanded-clause (process-hint cl hints state)))
       (value expanded-clause)))
 ;;  )
-
-;; ------------------------------------------------------------------------
-;;     Run translate-cmp on terms to generate translated terms
-(defsection translate-cmp-smtlink
-  :parents (Smtlink-process-user-hint)
-
-  (define wrld-fn-len ((cl t) (state))
-    :mode :program
-    (b* ((world (w state)))
-      (+ (acl2-count cl)
-         (len (remove-duplicates-eq
-               (strip-cadrs (universal-theory :here)))))))
-
-  (define trans-hypothesis ((val t) (state))
-    :mode :program
-    (b* (((unless (and (true-listp val)
-                       (car val)))
-          val)
-         ((mv err term)
-          (acl2::translate-cmp (car val) t t nil 'Smtlink-process-user-hint->trans-hypothesis
-                               (w state) (acl2::default-state-vars t)))
-         ((when err)
-          (er hard? 'Smtlink-process-user-hint->trans-hypothesis "Error ~
-    translating form: ~q0" (car val))))
-      `(,term ,@(cdr val))))
-
-  (define trans-hypothesis-list ((val t) (state))
-    :mode :program
-    (b* (((unless (true-listp val)) val)
-         ((unless (consp val)) val)
-         ((cons first rest) val)
-         (new-first (trans-hypothesis first state)))
-      (cons new-first (trans-hypothesis-list rest state))))
-
-  (define trans-argument ((val t))
-    :mode :program
-    (b* (((unless (and (true-listp val)
-                       (car val) (cadr val)))
-          val)
-         ((list* name type rest) val))
-      `(,name ,type ,@rest)))
-
-  (define trans-argument-list ((val t) (state))
-    :mode :program
-    (b* (((unless (true-listp val)) val)
-         ((unless (consp val)) val)
-         ((cons first rest) val)
-         (new-first (trans-argument first)))
-      (cons new-first (trans-argument-list rest state))))
-
-  (define trans-func-option ((opt t) (val t) (state))
-    :mode :program
-    (cond ((equal opt ':formals) (trans-argument-list val state))
-          ((equal opt ':returns) (trans-argument-list val state))
-          ((equal opt ':guard) (trans-hypothesis val state))
-          ((equal opt ':more-returns) (trans-hypothesis-list val state))
-          (t val)))
-
-  (define trans-function ((val t) (state))
-    :mode :program
-    (b* (((unless (and (true-listp val) (consp val)))
-          val)
-         ((list* first second rest) val)
-         (new-second (trans-func-option first second state))
-         (new-functions `(,first ,new-second ,@(trans-function rest state))))
-      new-functions))
-
-  (define trans-functions ((val t) (state))
-    :mode :program
-    (b* (((unless (true-listp val)) val)
-         ((unless (consp val)) val)
-         ((cons first rest) val)
-         ((cons fname options) first)
-         (new-first `(,fname ,@(trans-function options state))))
-      (cons new-first (trans-functions rest state))))
-
-  (define trans-kind-option ((opt t) (val t) (state))
-    :mode :program
-    (cond ((equal opt ':theorems) (trans-hypothesis-list val state))
-          (t val)))
-
-  (define trans-type-kind ((val t) (state))
-    :mode :program
-    (b* (((unless (and (true-listp val) (consp val)))
-          val)
-         ((list* first second rest) val)
-         (new-second (trans-kind-option first second state))
-         (new-kinds `(,first ,new-second ,@(trans-type-kind rest state))))
-      new-kinds))
-
-  (define trans-type-option ((opt t) (val t) (state))
-    :mode :program
-    (cond ((equal opt ':type) (trans-type-kind val state))
-          (t val)))
-
-  (define trans-type ((val t) state)
-    :mode :program
-    (b* (((unless (and (true-listp val) (consp val)))
-          val)
-         ((list* first second rest) val)
-         (new-second (trans-type-option first second state))
-         (new-types `(,first ,new-second ,@(trans-type rest state))))
-      new-types))
-
-  (define trans-types ((val t) (state))
-    :mode :program
-    (b* (((unless (true-listp val)) val)
-         ((unless (consp val)) val)
-         ((cons first rest) val)
-         ((cons typename options) first)
-         (new-first `(,typename ,@(trans-type options state))))
-      (cons new-first (trans-types rest state))))
-
-  (define trans-hint-option ((opt t) (val t) (state))
-    :mode :program
-    (cond ((equal opt ':functions) (trans-functions val state))
-          ((equal opt ':types) (trans-types val state))
-          ((equal opt ':hypotheses) (trans-hypothesis-list val state))
-          ((equal opt ':wrld-fn-len)
-           (er hard?
-               'Smtlink-process-user-hint->trans-hint-option
-               "User trying to access internal parameter ~
-                wrld-fn-len!"))
-          (t val)))
-
-  (define trans-hint ((cl t) (hint t) (state))
-    :mode :program
-    (b* (((unless (true-listp hint)) hint)
-         (wrld-len (wrld-fn-len cl state))
-         ((if (atom hint)) `(:wrld-fn-len ,wrld-len))
-         ((unless (cdr hint)) hint)
-         ((list* first second rest) hint)
-         (new-second (trans-hint-option first second state))
-         (new-hint `(,first ,new-second ,@(trans-hint cl rest state))))
-      new-hint))
-  )
 
 ;; ------------------------------------------------------------
 ;;         Prove correctness of clause processor
@@ -2011,18 +854,30 @@
                      b))
                (ev-smtcp (disjoin cl) b))
       :rule-classes :clause-processor))
+
+  (define wrld-fn-len ((cl t) (state))
+    :mode :program
+    (b* ((world (w state)))
+      (+ (acl2-count cl)
+         (len (remove-duplicates-eq
+               (strip-cadrs (universal-theory :here)))))))
+
   ;; Smtlink is a macro that generates a clause processor hint. This clause
   ;;   processor hint generates a clause, with which a new smt-hint is attached.
   ;;   This new smt-hint combines user given hints with hints from the state.
   ;; A computed hint will be waiting to take the clause and hint for clause
   ;;   expansion and transformation.
   (defmacro smtlink (clause hint)
-    `(process-hint-cp ,clause (trans-hint ,clause ',hint state) state))
+    `(b* ((len (wrld-fn-len clause state)))
+       (process-hint-cp ,clause
+                        (append ,hint `(:wrld-fn-len ,len))
+                        state)))
 
   (defmacro smtlink-custom (clause hint)
-    `(process-hint-cp ,clause
-                      (trans-hint ,clause ',(append hint '(:custom-p t)) state)
-                      state))
+    `(b* ((len (wrld-fn-len clause state)))
+       (process-hint-cp ,clause
+                        (append ,hint `(:wrld-fn-len ,len :customp t))
+                        state)))
 
   ;; Adding :smtlink as a custom :hints option
   (add-custom-keyword-hint :smtlink
