books/projects/smtlink/verified/expand-options.lisp
@@ -1,0 +1,72 @@
+;; Copyright (C) 2015, University of British Columbia
+;; Written by Yan Peng (April 19th 2021)
+;;
+;; License: A 3-clause BSD license.
+;; See the LICENSE file distributed with ACL2
+;;
+
+(in-package "SMT")
+(include-book "xdoc/top" :dir :system)
+(include-book "centaur/fty/top" :dir :system)
+
+(include-book "hint-interface")
+
+(defalist symbol-smt-function-alist
+  :key-type symbolp
+  :val-type smt-function-p
+  :pred symbol-smt-function-alistp
+  :true-listp t)
+
+(defthm assoc-equal-of-symbol-smt-function-alist
+  (implies (and (symbol-smt-function-alistp alst)
+                (assoc-equal x alst))
+           (and (consp (assoc-equal x alst))
+                (smt-function-p (cdr (assoc-equal x alst))))))
+
+(defprod expand-options
+  ((functions symbol-smt-function-alistp)
+   (types symbol-symbol-alistp)
+   (wrld-fn-len natp)))
+
+(define construct-function-info ((func-lst smt-function-list-p))
+  :returns (alst symbol-smt-function-alistp)
+  :measure (len func-lst)
+  (b* ((func-lst (smt-function-list-fix func-lst))
+       ((unless (consp func-lst)) nil)
+       ((cons func-hd func-tl) func-lst)
+       (name (smt-function->name func-hd)))
+    (acons name func-hd (construct-function-info func-tl))))
+
+(define construct-type-functions-helper ((func-lst smt-function-list-p)
+                                         (acc symbol-symbol-alistp))
+  :returns (alst symbol-symbol-alistp)
+  :measure (len func-lst)
+  (b* ((func-lst (smt-function-list-fix func-lst))
+       (acc (symbol-symbol-alist-fix acc))
+       ((unless (consp func-lst)) nil)
+       ((cons func-hd func-tl) func-lst)
+       (name (smt-function->name func-hd)))
+    (construct-type-functions-helper func-tl (acons name nil acc))))
+
+(define construct-type-functions ((types smt-type-list-p)
+                                  (acc symbol-symbol-alistp))
+  :returns (types symbol-symbol-alistp)
+  :measure (len types)
+  (b* ((types (smt-type-list-fix types))
+       (acc (symbol-symbol-alist-fix acc))
+       ((unless (consp types)) nil)
+       ((cons types-hd types-tl) types)
+       (acc-1 (acons (smt-type->recognizer types-hd) nil
+                     (construct-type-functions-helper
+                      (smt-type->functions types-hd) acc))))
+    (construct-type-functions types-tl acc-1)))
+
+(define construct-expand-options ((hints smtlink-hint-p))
+  :returns (eo expand-options-p)
+  (b* ((hints (smtlink-hint-fix hints))
+       ((smtlink-hint h) hints)
+       (functions (construct-function-info h.functions))
+       (types (construct-type-functions h.types nil)))
+    (make-expand-options :functions functions
+                         :types types
+                         :wrld-fn-len h.wrld-fn-len)))
