books/projects/smtlink/verified/hint-interface.lisp
@@ -18,134 +18,28 @@
 ;;   :parents (verified)
 ;;   :short "Define default Smtlink hint interface"
 
-(defprod hint-pair
-  :parents (smtlink-hint)
-  ((thm pseudo-termp "A theorem statement"
-        :default nil)
-   (hints true-listp "The ACL2 hint for proving this theorem"
-          :default nil)
-   (name symbolp "The name of the theorem if already proven in ACL2"
-         :default nil)))
+(defprod smt-return
+  ((var symbolp)
+   (thm symbolp)))
 
-(deflist hint-pair-list
-  :parents (hint-pair)
-  :elt-type hint-pair
-  :true-listp t)
-
-(defalist symbol-hint-pair-alist
-  :parents (hint-pair)
-  :key-type symbolp
-  :val-type hint-pair-p
-  :true-listp t)
-
-(defprod decl
-  :parents (smtlink-hint)
-  ((name symbolp :default nil)
-   (type hint-pair-p :default (make-hint-pair))
-   ;; The fixer should be found in types;
-   ;; So we don't need fixer in function hints.
-   ;; (fixer symbolp :default nil)
-   ))
-
-(deflist decl-list
-  :parents (decl)
-  :elt-type decl
+(deflist smt-return-list
+  :elt-type smt-return-p
   :true-listp t)
 
 (defprod smt-function
   :parents (smtlink-hint)
   ((name symbolp :default nil)
-   (expansion-depth natp :default 0)
-   (formals decl-list-p :default nil)
-   (returns decl-list-p :default nil)
-   ;; I'm not sure what's good of having guard,
-   ;; currently the hint is generated but is not used in Smtlink.
-   (guard hint-pair-p :default (make-hint-pair))
-   (more-returns hint-pair-list-p :default nil)))
+   (formals symbol-listp :default nil)
+   (returns smt-return-list-p :default nil)
+   (uninterpreted-hints true-listp :default nil)
+   (replace-thm symbolp :default nil)
+   (depth natp :default 0)))
 
 (defoption maybe-smt-function smt-function-p)
 
 (deflist smt-function-list
   :parents (smt-function)
   :elt-type smt-function-p
-  :true-listp t)
-
-(defprod type-thm
-  ((name symbolp :default nil)
-   (hints true-listp :default nil)))
-
-(defprod type-function
-  ((name symbolp :default nil)
-   (return-type symbolp :default nil)
-   (type-of-function-thm type-thm-p :default (make-type-thm))
-   (destructor-of-constructor-thm type-thm-p :default (make-type-thm))
-   ;; constructor doesn't use this field
-   ))
-
-(deflist type-function-list
-  :parents (type-function)
-  :elt-type type-function-p
-  :true-listp t)
-
-(defprod prod
-  ((kind symbolp :default nil)
-   (constructor type-function-p :default (make-type-function))
-   (destructors type-function-list-p :default nil)))
-
-(deflist prod-list
-  :elt-type prod-p
-  :true-listp t)
-
-(defalist symbol-prod-alist
-  :key-type symbolp
-  :val-type prod-p
-  :true-listp t)
-
-(deftagsum smt-type
-  (:abstract ())
-  (:array ((store type-function-p :default (make-type-function))
-           (select type-function-p :default (make-type-function))
-           (k type-function-p :default (make-type-function))
-           (key-type symbolp)
-           (val-type symbolp)
-           (array-thm type-thm-p :default (make-type-thm))))
-  ;; prod, list and option are all sums
-  (:sum ((kind-fn symbolp :default nil)
-         (prods prod-list-p :default nil)))
-  )
-
-(define smt-type-kind-fn ((smt-type smt-type-p))
-  :guard (equal (smt-type-kind smt-type) :sum)
-  (b* ((smt-type (smt-type-fix smt-type))
-       (kind-fn (smt-type-sum->kind-fn smt-type))
-       ((if (null kind-fn)) 'kind))
-    kind-fn))
-
-(defprod smt-fixtype
-  :parents (smtlink-hint)
-  ((name symbolp :default nil)
-   (recognizer symbolp :default nil)
-   (fixer symbolp :default nil)
-   (fixer-when-recognizer-thm type-thm-p :default (make-type-thm))
-   (basicp symbolp :default nil)
-   (kind smt-type-p :default (make-smt-type-abstract))))
-
-(defoption maybe-smt-fixtype smt-fixtype-p)
-
-(deflist smt-fixtype-list
-  :parents (smt-fixtype)
-  :elt-type smt-fixtype-p
-  :true-listp t)
-
-(defprod info-pair
-  ((name symbolp)
-   (fn-type symbolp)
-   (kind symbolp))) ;; :store, :select, :recognizer, :fixer, :constructor,
-;; :destructor, :kind-fn
-
-(defalist smt-fixtype-info
-  :key-type symbolp ;; function name
-  :val-type info-pair-p
   :true-listp t)
 
 (defprod smt-config
@@ -158,23 +52,36 @@
   (:switch ((okp booleanp :default nil)))
   (:symbol-list ((lst symbol-listp :default nil))))
 
+(defprod smt-hypo
+  ((thm symbolp)
+   (subst symbol-pseudo-term-alistp)))
+
+(deflist smt-hypo-list
+  :elt-type smt-hypo-p
+  :true-listp t)
+
+(defprod smt-type
+  ((recognizer symbolp)
+   (functions smt-function-list-p)
+   (subtypes symbol-listp)))
+
+(deflist smt-type-list
+  :elt-type smt-type-p
+  :true-listp t)
+
 (local (in-theory (disable symbol-listp)))
 
 (defprod smtlink-hint
   :parents (SMT-hint-interface)
   ((functions smt-function-list-p :default nil)
-   (types smt-fixtype-list-p :default nil)
-   (types-info smt-fixtype-info-p :default nil)
-   (hypotheses hint-pair-list-p :default nil)
+   (types smt-type-list-p :default nil)
+   (hypotheses smt-hypo-list-p :default nil)
    (configurations smt-config-p :default (make-smt-config))
-
-   (int-to-rat int-to-rat-p :default (make-int-to-rat-switch :okp nil))
-   (use-uninterpreted booleanp :default t)
-   (under-induct symbolp :default nil)
+   (int-to-ratp int-to-rat-p :default (make-int-to-rat-switch :okp nil))
+   (under-inductionp symbolp :default nil)
    (global-hint symbolp :default nil)
    (wrld-fn-len natp :default 0)
-   (custom-p booleanp :default nil)
-   ))
+   (customp booleanp :default nil)))
 
 (defalist smtlink-hint-alist
   :key-type symbolp
@@ -182,259 +89,6 @@
   :true-listp t)
 
 (defthm assoc-equal-of-smtlink-hint-alist
-  (implies (and (smtlink-hint-alist-p x)
-                (consp (assoc-equal name x)))
-           (and (smtlink-hint-p (cdr (assoc-equal name x)))
-                (cdr (assoc-equal name x)))))
-;; ---------------------------------------------------------------
-;; Utility functions
-
-;; decl-list functions
-(define get-thm-from-decl ((decl decl-p))
-  :returns (thm pseudo-termp)
-  (hint-pair->thm (decl->type (decl-fix decl))))
-
-(define get-thms-from-decl-list ((dlst decl-list-p))
-  :returns (thms pseudo-term-listp)
-  :measure (len dlst)
-  (b* ((dlst (decl-list-fix dlst))
-       ((unless (consp dlst)) nil)
-       ((cons first rest) dlst))
-    (cons (get-thm-from-decl first)
-          (get-thms-from-decl-list rest))))
-
-;; smt-function-list functions
-(define is-function ((name symbolp) (fn-lst smt-function-list-p))
-  :returns (f maybe-smt-function-p)
-  :measure (len fn-lst)
-  (b* ((fn-lst (smt-function-list-fix fn-lst))
-       ((unless (consp fn-lst)) nil)
-       ((cons first rest) fn-lst)
-       (first-name (smt-function->name first))
-       ((if (equal first-name name)) first))
-    (is-function name rest)))
-
-;; smt-fixtype-list functions
-(define generate-info-pair ((fn symbolp)
-                            (name symbolp)
-                            (fn-type symbolp)
-                            (kind symbolp)
-                            (acc smt-fixtype-info-p))
-  :returns (info smt-fixtype-info-p)
-  (b* ((fn (symbol-fix fn))
-       (name (symbol-fix name))
-       (kind (symbol-fix kind))
-       (fn-type (symbol-fix fn-type))
-       (acc (smt-fixtype-info-fix acc)))
-    (acons fn
-           (make-info-pair :name name
-                           :fn-type fn-type
-                           :kind kind)
-           acc)))
-
-(define generate-fixtype-info-array ((name symbolp)
-                                     (type smt-type-p)
-                                     (acc smt-fixtype-info-p))
-  :returns (info smt-fixtype-info-p)
-  :guard (equal (smt-type-kind type) :array)
-  (b* ((name (symbol-fix name))
-       (type (smt-type-fix type))
-       (acc (smt-fixtype-info-fix acc))
-       ((smt-type-array a) type)
-       (store-acc (generate-info-pair (type-function->name a.store)
-                                      name :store nil acc)))
-    (generate-info-pair (type-function->name a.select) name :select nil store-acc)))
-
-(define generate-fixtype-info-destructors ((name symbolp)
-                                           (kind symbolp)
-                                           (destructors type-function-list-p)
-                                           (acc smt-fixtype-info-p))
-  :returns (info smt-fixtype-info-p)
-  :measure (len destructors)
-  (b* ((name (symbol-fix name))
-       (kind (symbol-fix kind))
-       (destructors (type-function-list-fix destructors))
-       (acc (smt-fixtype-info-fix acc))
-       ((unless (consp destructors)) acc)
-       ((cons first rest) destructors)
-       ((type-function f) first)
-       (first-acc (generate-info-pair f.name name :destructor kind acc)))
-    (generate-fixtype-info-destructors name kind rest first-acc)))
-
-(define generate-fixtype-info-prod ((name symbolp)
-                                    (prod prod-p)
-                                    (acc smt-fixtype-info-p))
-  :returns (info smt-fixtype-info-p)
-  (b* ((name (symbol-fix name))
-       (prod (prod-fix prod))
-       ((prod p) prod)
-       (acc (smt-fixtype-info-fix acc))
-       (constructor-acc
-        (generate-info-pair (type-function->name p.constructor)
-                            name :constructor p.kind acc)))
-    (generate-fixtype-info-destructors name p.kind p.destructors
-                                       constructor-acc)))
-
-(define generate-fixtype-info-prod-list ((name symbolp)
-                                         (prods prod-list-p)
-                                         (acc smt-fixtype-info-p))
-  :returns (info smt-fixtype-info-p)
-  :measure (len prods)
-  (b* ((name (symbol-fix name))
-       (prods (prod-list-fix prods))
-       (acc (smt-fixtype-info-fix acc))
-       ((unless (consp prods)) acc)
-       ((cons first rest) prods)
-       (first-acc (generate-fixtype-info-prod name first acc)))
-    (generate-fixtype-info-prod-list name rest first-acc)))
-
-(define generate-fixtype-info-sum ((name symbolp)
-                                   (type smt-type-p)
-                                   (acc smt-fixtype-info-p))
-  :returns (info smt-fixtype-info-p)
-  :guard (equal (smt-type-kind type) :sum)
-  (b* ((type (smt-type-fix type))
-       (acc (smt-fixtype-info-fix acc))
-       ((smt-type-sum s) type)
-       ((if (null s.kind-fn))
-        (generate-fixtype-info-prod-list name s.prods acc))
-       (new-acc (generate-info-pair s.kind-fn name :kind-fn nil acc)))
-    (generate-fixtype-info-prod-list name s.prods new-acc)))
-
-(define generate-fixtype-info-kind ((name symbolp)
-                                    (type smt-type-p)
-                                    (acc smt-fixtype-info-p))
-  :returns (info smt-fixtype-info-p)
-  (b* ((type (smt-type-fix type))
-       (acc (smt-fixtype-info-fix acc))
-       (kind (smt-type-kind type)))
-    (case kind
-      (:array (generate-fixtype-info-array name type acc))
-      (:sum (generate-fixtype-info-sum name type acc))
-      (:abstract acc))))
-
-(define generate-one-fixtype-info ((type smt-fixtype-p)
-                                   (acc smt-fixtype-info-p))
-  :returns (info smt-fixtype-info-p)
-  (b* ((type (smt-fixtype-fix type))
-       (acc (smt-fixtype-info-fix acc))
-       ((smt-fixtype f) type)
-       (rec-acc (generate-info-pair f.recognizer f.name :recognizer nil acc))
-       (fix-acc (generate-info-pair f.fixer f.name :fixer nil rec-acc)))
-    (generate-fixtype-info-kind f.name f.kind fix-acc)))
-
-(define generate-fixtype-info ((types smt-fixtype-list-p)
-                               (acc smt-fixtype-info-p))
-  :returns (info smt-fixtype-info-p)
-  :measure (len types)
-  (b* ((types (smt-fixtype-list-fix types))
-       (acc (smt-fixtype-info-fix acc))
-       ((unless (consp types)) acc)
-       ((cons first rest) types)
-       (new-acc (generate-one-fixtype-info first acc)))
-    (generate-fixtype-info rest new-acc)))
-
-(define add-fixtype-info ((hint smtlink-hint-p))
-  :returns (new-hint smtlink-hint-p)
-  (b* ((hint (smtlink-hint-fix hint))
-       ((smtlink-hint h) hint)
-       (info (generate-fixtype-info h.types nil)))
-    (change-smtlink-hint hint :types-info info)))
-
-(define is-type ((x symbolp) (fixtypes smt-fixtype-list-p))
-  :returns (type maybe-smt-fixtype-p)
-  :measure (len fixtypes)
-  (b* ((fixtypes (smt-fixtype-list-fix fixtypes))
-       ((unless (consp fixtypes)) nil)
-       ((cons first rest) fixtypes)
-       ((if (equal x (smt-fixtype->recognizer first))) first))
-    (is-type x rest)))
-
-(define is-recognizer ((x symbolp) (fixinfo smt-fixtype-info-p))
-  :returns (okp booleanp)
-  (b* ((fixinfo (smt-fixtype-info-fix fixinfo))
-       (item (assoc-equal x fixinfo))
-       ((unless item) nil)
-       ((info-pair p) (cdr item)))
-    (equal p.fn-type :recognizer)))
-
-(define is-fixer ((x symbolp) (fixinfo smt-fixtype-info-p))
-  :returns (okp booleanp)
-  (b* ((fixinfo (smt-fixtype-info-fix fixinfo))
-       (item (assoc-equal x fixinfo))
-       ((unless item) nil)
-       ((info-pair p) (cdr item)))
-    (equal p.fn-type :fixer)))
-
-(define name-of-recognizer ((x symbolp) (fixinfo smt-fixtype-info-p))
-  :returns (name symbolp)
-  (b* ((fixinfo (smt-fixtype-info-fix fixinfo))
-       (item (assoc-equal x fixinfo))
-       ((unless item) nil)
-       ((info-pair p) (cdr item)))
-    p.name))
-
-(define fncall-of-fixtypes ((x symbolp) (fixinfo smt-fixtype-info-p))
-  :returns (ok booleanp)
-  (b* ((fixinfo (smt-fixtype-info-fix fixinfo)))
-    (not (null (assoc-equal x fixinfo)))))
-
-(define fixer-of-recognizer ((x symbolp) (fixtypes smt-fixtype-list-p))
-  :returns (fixer symbolp)
-  :measure (len fixtypes)
-  (b* ((fixtypes (smt-fixtype-list-fix fixtypes))
-       ((unless (consp fixtypes)) nil)
-       ((cons first rest) fixtypes)
-       ((if (equal x (smt-fixtype->recognizer first)))
-        (smt-fixtype->fixer first)))
-    (fixer-of-recognizer x rest)))
-
-(define recognizer-of-fixer ((x symbolp) (fixtypes smt-fixtype-list-p))
-  :returns (recognizer symbolp)
-  :measure (len fixtypes)
-  (b* ((fixtypes (smt-fixtype-list-fix fixtypes))
-       ((unless (consp fixtypes)) nil)
-       ((cons first rest) fixtypes)
-       ((if (equal x (smt-fixtype->fixer first)))
-        (smt-fixtype->recognizer first)))
-    (recognizer-of-fixer x rest)))
-
-(define type-decl-p ((expr pseudo-termp)
-                     (fixinfo smt-fixtype-info-p))
-  :returns (is-decl? booleanp)
-  (b* (;; ((if (is-type-hyp-decl expr)) t)
-       ((unless (equal (len expr) 2))
-        nil)
-       (fn-name (car expr))
-       ((unless (symbolp fn-name)) nil)
-       ((unless (is-recognizer fn-name fixinfo))
-        nil)
-       ((unless (and (symbolp (cadr expr)) (cadr expr))) nil))
-    t)
-  ///
-  (more-returns
-   (is-decl?
-    (implies is-decl?
-             (and (consp expr)
-                  (consp (cdr expr))
-                  (symbolp (car expr))
-                  (is-recognizer (car expr) fixinfo)
-                  (symbolp (cadr expr)) (cadr expr)))
-    :name type-decl-p-definition)))
-
-(define return-type-of-function ((f smt-function-p)
-                                 (fixinfo smt-fixtype-info-p))
-  :returns (type symbolp)
-  (b* ((f (smt-function-fix f))
-       ((smt-function f) f)
-       ((unless (and (consp f.returns)
-                     (null (cdr f.returns))))
-        (er hard? 'hint-interface=>return-type-of-function
-            "Smtlink only supports functions that return one value, but ~p0
-    returns two: ~p1~%" f.name f.returns))
-       (type-thm (hint-pair->thm (decl->type (car f.returns))))
-       ((unless (type-decl-p type-thm fixinfo))
-        (er hard? 'hint-interface=>return-type-of-function
-            "Not a type declaration: ~p0~%" type-thm)))
-    (car type-thm)))
-;;  )
+  (implies (and (smtlink-hint-alist-p alst)
+                (assoc-equal x alst))
+           (smtlink-hint-p (cdr (assoc-equal x alst)))))
